src/FcEtt/ett_ott.v
@@ -7,20 +7,26 @@ Definition const := atom.
 Definition tyfam := atom.
 Definition index := nat. (*r indices *)
 
+Inductive role : Set :=  (*r Role *)
+ | Nom : role
+ | Rep : role.
+
 Inductive relflag : Set :=  (*r relevance flag *)
  | Rel : relflag
  | Irrel : relflag.
 
-Inductive tm : Set :=  (*r types and kinds *)
+Inductive constraint : Set :=  (*r props *)
+ | Eq (a:tm) (b:tm) (A:tm) (R:role)
+with tm : Set :=  (*r types and kinds *)
  | a_Star : tm
  | a_Var_b (_:nat)
  | a_Var_f (x:tmvar)
- | a_Abs (rho:relflag) (A:tm) (b:tm)
+ | a_Abs (rho:relflag) (A:tm) (R:role) (b:tm)
  | a_UAbs (rho:relflag) (b:tm)
  | a_App (a:tm) (rho:relflag) (b:tm)
  | a_Fam (F:tyfam)
  | a_Const (T:const)
- | a_Pi (rho:relflag) (A:tm) (B:tm)
+ | a_Pi (rho:relflag) (A:tm) (R:role) (B:tm)
  | a_Conv (a:tm) (g:co)
  | a_CPi (phi:constraint) (B:tm)
  | a_CAbs (phi:constraint) (b:tm)
@@ -53,27 +59,25 @@ with co : Set :=  (*r explicit coercions *)
  | g_CAppCong (g:co) (g1:co) (g2:co)
  | g_CPiSnd (g:co) (g1:co) (g2:co)
  | g_Cast (g1:co) (g2:co)
- | g_EqCong (g1:co) (A:tm) (g2:co)
+ | g_EqCong (g1:co) (A:tm) (R:role) (g2:co)
  | g_IsoConv (phi1:constraint) (phi2:constraint) (g:co)
  | g_Eta (a:tm)
  | g_Left (g:co) (g':co)
- | g_Right (g:co) (g':co)
-with constraint : Set :=  (*r props *)
- | Eq (a:tm) (b:tm) (A:tm).
+ | g_Right (g:co) (g':co).
 
 Inductive sort : Set :=  (*r binding classifier *)
- | Tm (A:tm)
+ | Tm (A:tm) (R:role)
  | Co (phi:constraint).
 
 Inductive sig_sort : Set :=  (*r signature classifier *)
  | Cs (A:tm)
- | Ax (a:tm) (A:tm).
+ | Ax (a:tm) (A:tm) (R:role).
 
 Definition context : Set := list ( atom * sort ).
 
-Definition available_props : Type := atoms.
-
 Definition sig : Set := list (atom * sig_sort).
+
+Definition available_props : Type := atoms.
 
 (* EXPERIMENTAL *)
 (** auxiliary functions on the new list types *)
@@ -81,99 +85,7 @@ Definition sig : Set := list (atom * sig_sort).
 (** subrules *)
 (** arities *)
 (** opening up abstractions *)
-Fixpoint open_brs_wrt_tm_rec (k:nat) (a5:tm) (brs_6:brs) {struct brs_6}: brs :=
-  match brs_6 with
-  | br_None => br_None 
-  | (br_One K a brs5) => br_One K (open_tm_wrt_tm_rec k a5 a) (open_brs_wrt_tm_rec k a5 brs5)
-end
-with open_tm_wrt_tm_rec (k:nat) (a5:tm) (a_6:tm) {struct a_6}: tm :=
-  match a_6 with
-  | a_Star => a_Star 
-  | (a_Var_b nat) => 
-      match lt_eq_lt_dec nat k with
-        | inleft (left _) => a_Var_b nat
-        | inleft (right _) => a5
-        | inright _ => a_Var_b (nat - 1)
-      end
-  | (a_Var_f x) => a_Var_f x
-  | (a_Abs rho A b) => a_Abs rho (open_tm_wrt_tm_rec k a5 A) (open_tm_wrt_tm_rec (S k) a5 b)
-  | (a_UAbs rho b) => a_UAbs rho (open_tm_wrt_tm_rec (S k) a5 b)
-  | (a_App a rho b) => a_App (open_tm_wrt_tm_rec k a5 a) rho (open_tm_wrt_tm_rec k a5 b)
-  | (a_Fam F) => a_Fam F
-  | (a_Const T) => a_Const T
-  | (a_Pi rho A B) => a_Pi rho (open_tm_wrt_tm_rec k a5 A) (open_tm_wrt_tm_rec (S k) a5 B)
-  | (a_Conv a g) => a_Conv (open_tm_wrt_tm_rec k a5 a) (open_co_wrt_tm_rec k a5 g)
-  | (a_CPi phi B) => a_CPi (open_constraint_wrt_tm_rec k a5 phi) (open_tm_wrt_tm_rec k a5 B)
-  | (a_CAbs phi b) => a_CAbs (open_constraint_wrt_tm_rec k a5 phi) (open_tm_wrt_tm_rec k a5 b)
-  | (a_UCAbs b) => a_UCAbs (open_tm_wrt_tm_rec k a5 b)
-  | (a_CApp a g) => a_CApp (open_tm_wrt_tm_rec k a5 a) (open_co_wrt_tm_rec k a5 g)
-  | a_Bullet => a_Bullet 
-  | (a_DataCon K) => a_DataCon K
-  | (a_Case a brs5) => a_Case (open_tm_wrt_tm_rec k a5 a) (open_brs_wrt_tm_rec k a5 brs5)
-end
-with open_constraint_wrt_tm_rec (k:nat) (a5:tm) (phi5:constraint) : constraint :=
-  match phi5 with
-  | (Eq a b A) => Eq (open_tm_wrt_tm_rec k a5 a) (open_tm_wrt_tm_rec k a5 b) (open_tm_wrt_tm_rec k a5 A)
-end
-with open_co_wrt_tm_rec (k:nat) (a5:tm) (g_5:co) {struct g_5}: co :=
-  match g_5 with
-  | g_Triv => g_Triv 
-  | (g_Var_b nat) => g_Var_b nat
-  | (g_Var_f c) => g_Var_f c
-  | (g_Beta a b) => g_Beta (open_tm_wrt_tm_rec k a5 a) (open_tm_wrt_tm_rec k a5 b)
-  | (g_Refl a) => g_Refl (open_tm_wrt_tm_rec k a5 a)
-  | (g_Refl2 a b g) => g_Refl2 (open_tm_wrt_tm_rec k a5 a) (open_tm_wrt_tm_rec k a5 b) (open_co_wrt_tm_rec k a5 g)
-  | (g_Sym g) => g_Sym (open_co_wrt_tm_rec k a5 g)
-  | (g_Trans g1 g2) => g_Trans (open_co_wrt_tm_rec k a5 g1) (open_co_wrt_tm_rec k a5 g2)
-  | (g_PiCong rho g1 g2) => g_PiCong rho (open_co_wrt_tm_rec k a5 g1) (open_co_wrt_tm_rec (S k) a5 g2)
-  | (g_AbsCong rho g1 g2) => g_AbsCong rho (open_co_wrt_tm_rec k a5 g1) (open_co_wrt_tm_rec (S k) a5 g2)
-  | (g_AppCong g1 rho g2) => g_AppCong (open_co_wrt_tm_rec k a5 g1) rho (open_co_wrt_tm_rec k a5 g2)
-  | (g_PiFst g) => g_PiFst (open_co_wrt_tm_rec k a5 g)
-  | (g_CPiFst g) => g_CPiFst (open_co_wrt_tm_rec k a5 g)
-  | (g_IsoSnd g) => g_IsoSnd (open_co_wrt_tm_rec k a5 g)
-  | (g_PiSnd g1 g2) => g_PiSnd (open_co_wrt_tm_rec k a5 g1) (open_co_wrt_tm_rec k a5 g2)
-  | (g_CPiCong g1 g3) => g_CPiCong (open_co_wrt_tm_rec k a5 g1) (open_co_wrt_tm_rec k a5 g3)
-  | (g_CAbsCong g1 g3 g4) => g_CAbsCong (open_co_wrt_tm_rec k a5 g1) (open_co_wrt_tm_rec k a5 g3) (open_co_wrt_tm_rec k a5 g4)
-  | (g_CAppCong g g1 g2) => g_CAppCong (open_co_wrt_tm_rec k a5 g) (open_co_wrt_tm_rec k a5 g1) (open_co_wrt_tm_rec k a5 g2)
-  | (g_CPiSnd g g1 g2) => g_CPiSnd (open_co_wrt_tm_rec k a5 g) (open_co_wrt_tm_rec k a5 g1) (open_co_wrt_tm_rec k a5 g2)
-  | (g_Cast g1 g2) => g_Cast (open_co_wrt_tm_rec k a5 g1) (open_co_wrt_tm_rec k a5 g2)
-  | (g_EqCong g1 A g2) => g_EqCong (open_co_wrt_tm_rec k a5 g1) (open_tm_wrt_tm_rec k a5 A) (open_co_wrt_tm_rec k a5 g2)
-  | (g_IsoConv phi1 phi2 g) => g_IsoConv (open_constraint_wrt_tm_rec k a5 phi1) (open_constraint_wrt_tm_rec k a5 phi2) (open_co_wrt_tm_rec k a5 g)
-  | (g_Eta a) => g_Eta (open_tm_wrt_tm_rec k a5 a)
-  | (g_Left g g') => g_Left (open_co_wrt_tm_rec k a5 g) (open_co_wrt_tm_rec k a5 g')
-  | (g_Right g g') => g_Right (open_co_wrt_tm_rec k a5 g) (open_co_wrt_tm_rec k a5 g')
-end.
-
-Fixpoint open_brs_wrt_co_rec (k:nat) (g5:co) (brs_6:brs) {struct brs_6}: brs :=
-  match brs_6 with
-  | br_None => br_None 
-  | (br_One K a brs5) => br_One K (open_tm_wrt_co_rec k g5 a) (open_brs_wrt_co_rec k g5 brs5)
-end
-with open_tm_wrt_co_rec (k:nat) (g5:co) (a5:tm) {struct a5}: tm :=
-  match a5 with
-  | a_Star => a_Star 
-  | (a_Var_b nat) => a_Var_b nat
-  | (a_Var_f x) => a_Var_f x
-  | (a_Abs rho A b) => a_Abs rho (open_tm_wrt_co_rec k g5 A) (open_tm_wrt_co_rec k g5 b)
-  | (a_UAbs rho b) => a_UAbs rho (open_tm_wrt_co_rec k g5 b)
-  | (a_App a rho b) => a_App (open_tm_wrt_co_rec k g5 a) rho (open_tm_wrt_co_rec k g5 b)
-  | (a_Fam F) => a_Fam F
-  | (a_Const T) => a_Const T
-  | (a_Pi rho A B) => a_Pi rho (open_tm_wrt_co_rec k g5 A) (open_tm_wrt_co_rec k g5 B)
-  | (a_Conv a g) => a_Conv (open_tm_wrt_co_rec k g5 a) (open_co_wrt_co_rec k g5 g)
-  | (a_CPi phi B) => a_CPi (open_constraint_wrt_co_rec k g5 phi) (open_tm_wrt_co_rec (S k) g5 B)
-  | (a_CAbs phi b) => a_CAbs (open_constraint_wrt_co_rec k g5 phi) (open_tm_wrt_co_rec (S k) g5 b)
-  | (a_UCAbs b) => a_UCAbs (open_tm_wrt_co_rec (S k) g5 b)
-  | (a_CApp a g) => a_CApp (open_tm_wrt_co_rec k g5 a) (open_co_wrt_co_rec k g5 g)
-  | a_Bullet => a_Bullet 
-  | (a_DataCon K) => a_DataCon K
-  | (a_Case a brs5) => a_Case (open_tm_wrt_co_rec k g5 a) (open_brs_wrt_co_rec k g5 brs5)
-end
-with open_constraint_wrt_co_rec (k:nat) (g5:co) (phi5:constraint) : constraint :=
-  match phi5 with
-  | (Eq a b A) => Eq (open_tm_wrt_co_rec k g5 a) (open_tm_wrt_co_rec k g5 b) (open_tm_wrt_co_rec k g5 A)
-end
-with open_co_wrt_co_rec (k:nat) (g_5:co) (g__6:co) {struct g__6}: co :=
+Fixpoint open_co_wrt_co_rec (k:nat) (g_5:co) (g__6:co) {struct g__6}: co :=
   match g__6 with
   | g_Triv => g_Triv 
   | (g_Var_b nat) => 
@@ -200,72 +112,158 @@ with open_co_wrt_co_rec (k:nat) (g_5:co) (g__6:co) {struct g__6}: co :=
   | (g_CAppCong g g1 g2) => g_CAppCong (open_co_wrt_co_rec k g_5 g) (open_co_wrt_co_rec k g_5 g1) (open_co_wrt_co_rec k g_5 g2)
   | (g_CPiSnd g g1 g2) => g_CPiSnd (open_co_wrt_co_rec k g_5 g) (open_co_wrt_co_rec k g_5 g1) (open_co_wrt_co_rec k g_5 g2)
   | (g_Cast g1 g2) => g_Cast (open_co_wrt_co_rec k g_5 g1) (open_co_wrt_co_rec k g_5 g2)
-  | (g_EqCong g1 A g2) => g_EqCong (open_co_wrt_co_rec k g_5 g1) (open_tm_wrt_co_rec k g_5 A) (open_co_wrt_co_rec k g_5 g2)
+  | (g_EqCong g1 A R g2) => g_EqCong (open_co_wrt_co_rec k g_5 g1) (open_tm_wrt_co_rec k g_5 A) R (open_co_wrt_co_rec k g_5 g2)
   | (g_IsoConv phi1 phi2 g) => g_IsoConv (open_constraint_wrt_co_rec k g_5 phi1) (open_constraint_wrt_co_rec k g_5 phi2) (open_co_wrt_co_rec k g_5 g)
   | (g_Eta a) => g_Eta (open_tm_wrt_co_rec k g_5 a)
   | (g_Left g g') => g_Left (open_co_wrt_co_rec k g_5 g) (open_co_wrt_co_rec k g_5 g')
   | (g_Right g g') => g_Right (open_co_wrt_co_rec k g_5 g) (open_co_wrt_co_rec k g_5 g')
+end
+with open_brs_wrt_co_rec (k:nat) (g5:co) (brs_6:brs) {struct brs_6}: brs :=
+  match brs_6 with
+  | br_None => br_None 
+  | (br_One K a brs5) => br_One K (open_tm_wrt_co_rec k g5 a) (open_brs_wrt_co_rec k g5 brs5)
+end
+with open_tm_wrt_co_rec (k:nat) (g5:co) (a5:tm) {struct a5}: tm :=
+  match a5 with
+  | a_Star => a_Star 
+  | (a_Var_b nat) => a_Var_b nat
+  | (a_Var_f x) => a_Var_f x
+  | (a_Abs rho A R b) => a_Abs rho (open_tm_wrt_co_rec k g5 A) R (open_tm_wrt_co_rec k g5 b)
+  | (a_UAbs rho b) => a_UAbs rho (open_tm_wrt_co_rec k g5 b)
+  | (a_App a rho b) => a_App (open_tm_wrt_co_rec k g5 a) rho (open_tm_wrt_co_rec k g5 b)
+  | (a_Fam F) => a_Fam F
+  | (a_Const T) => a_Const T
+  | (a_Pi rho A R B) => a_Pi rho (open_tm_wrt_co_rec k g5 A) R (open_tm_wrt_co_rec k g5 B)
+  | (a_Conv a g) => a_Conv (open_tm_wrt_co_rec k g5 a) (open_co_wrt_co_rec k g5 g)
+  | (a_CPi phi B) => a_CPi (open_constraint_wrt_co_rec k g5 phi) (open_tm_wrt_co_rec (S k) g5 B)
+  | (a_CAbs phi b) => a_CAbs (open_constraint_wrt_co_rec k g5 phi) (open_tm_wrt_co_rec (S k) g5 b)
+  | (a_UCAbs b) => a_UCAbs (open_tm_wrt_co_rec (S k) g5 b)
+  | (a_CApp a g) => a_CApp (open_tm_wrt_co_rec k g5 a) (open_co_wrt_co_rec k g5 g)
+  | a_Bullet => a_Bullet 
+  | (a_DataCon K) => a_DataCon K
+  | (a_Case a brs5) => a_Case (open_tm_wrt_co_rec k g5 a) (open_brs_wrt_co_rec k g5 brs5)
+end
+with open_constraint_wrt_co_rec (k:nat) (g5:co) (phi5:constraint) : constraint :=
+  match phi5 with
+  | (Eq a b A R) => Eq (open_tm_wrt_co_rec k g5 a) (open_tm_wrt_co_rec k g5 b) (open_tm_wrt_co_rec k g5 A) R
 end.
 
-Definition open_sort_wrt_tm_rec (k:nat) (a5:tm) (sort5:sort) : sort :=
+Fixpoint open_co_wrt_tm_rec (k:nat) (a5:tm) (g_5:co) {struct g_5}: co :=
+  match g_5 with
+  | g_Triv => g_Triv 
+  | (g_Var_b nat) => g_Var_b nat
+  | (g_Var_f c) => g_Var_f c
+  | (g_Beta a b) => g_Beta (open_tm_wrt_tm_rec k a5 a) (open_tm_wrt_tm_rec k a5 b)
+  | (g_Refl a) => g_Refl (open_tm_wrt_tm_rec k a5 a)
+  | (g_Refl2 a b g) => g_Refl2 (open_tm_wrt_tm_rec k a5 a) (open_tm_wrt_tm_rec k a5 b) (open_co_wrt_tm_rec k a5 g)
+  | (g_Sym g) => g_Sym (open_co_wrt_tm_rec k a5 g)
+  | (g_Trans g1 g2) => g_Trans (open_co_wrt_tm_rec k a5 g1) (open_co_wrt_tm_rec k a5 g2)
+  | (g_PiCong rho g1 g2) => g_PiCong rho (open_co_wrt_tm_rec k a5 g1) (open_co_wrt_tm_rec (S k) a5 g2)
+  | (g_AbsCong rho g1 g2) => g_AbsCong rho (open_co_wrt_tm_rec k a5 g1) (open_co_wrt_tm_rec (S k) a5 g2)
+  | (g_AppCong g1 rho g2) => g_AppCong (open_co_wrt_tm_rec k a5 g1) rho (open_co_wrt_tm_rec k a5 g2)
+  | (g_PiFst g) => g_PiFst (open_co_wrt_tm_rec k a5 g)
+  | (g_CPiFst g) => g_CPiFst (open_co_wrt_tm_rec k a5 g)
+  | (g_IsoSnd g) => g_IsoSnd (open_co_wrt_tm_rec k a5 g)
+  | (g_PiSnd g1 g2) => g_PiSnd (open_co_wrt_tm_rec k a5 g1) (open_co_wrt_tm_rec k a5 g2)
+  | (g_CPiCong g1 g3) => g_CPiCong (open_co_wrt_tm_rec k a5 g1) (open_co_wrt_tm_rec k a5 g3)
+  | (g_CAbsCong g1 g3 g4) => g_CAbsCong (open_co_wrt_tm_rec k a5 g1) (open_co_wrt_tm_rec k a5 g3) (open_co_wrt_tm_rec k a5 g4)
+  | (g_CAppCong g g1 g2) => g_CAppCong (open_co_wrt_tm_rec k a5 g) (open_co_wrt_tm_rec k a5 g1) (open_co_wrt_tm_rec k a5 g2)
+  | (g_CPiSnd g g1 g2) => g_CPiSnd (open_co_wrt_tm_rec k a5 g) (open_co_wrt_tm_rec k a5 g1) (open_co_wrt_tm_rec k a5 g2)
+  | (g_Cast g1 g2) => g_Cast (open_co_wrt_tm_rec k a5 g1) (open_co_wrt_tm_rec k a5 g2)
+  | (g_EqCong g1 A R g2) => g_EqCong (open_co_wrt_tm_rec k a5 g1) (open_tm_wrt_tm_rec k a5 A) R (open_co_wrt_tm_rec k a5 g2)
+  | (g_IsoConv phi1 phi2 g) => g_IsoConv (open_constraint_wrt_tm_rec k a5 phi1) (open_constraint_wrt_tm_rec k a5 phi2) (open_co_wrt_tm_rec k a5 g)
+  | (g_Eta a) => g_Eta (open_tm_wrt_tm_rec k a5 a)
+  | (g_Left g g') => g_Left (open_co_wrt_tm_rec k a5 g) (open_co_wrt_tm_rec k a5 g')
+  | (g_Right g g') => g_Right (open_co_wrt_tm_rec k a5 g) (open_co_wrt_tm_rec k a5 g')
+end
+with open_brs_wrt_tm_rec (k:nat) (a5:tm) (brs_6:brs) {struct brs_6}: brs :=
+  match brs_6 with
+  | br_None => br_None 
+  | (br_One K a brs5) => br_One K (open_tm_wrt_tm_rec k a5 a) (open_brs_wrt_tm_rec k a5 brs5)
+end
+with open_tm_wrt_tm_rec (k:nat) (a5:tm) (a_6:tm) {struct a_6}: tm :=
+  match a_6 with
+  | a_Star => a_Star 
+  | (a_Var_b nat) => 
+      match lt_eq_lt_dec nat k with
+        | inleft (left _) => a_Var_b nat
+        | inleft (right _) => a5
+        | inright _ => a_Var_b (nat - 1)
+      end
+  | (a_Var_f x) => a_Var_f x
+  | (a_Abs rho A R b) => a_Abs rho (open_tm_wrt_tm_rec k a5 A) R (open_tm_wrt_tm_rec (S k) a5 b)
+  | (a_UAbs rho b) => a_UAbs rho (open_tm_wrt_tm_rec (S k) a5 b)
+  | (a_App a rho b) => a_App (open_tm_wrt_tm_rec k a5 a) rho (open_tm_wrt_tm_rec k a5 b)
+  | (a_Fam F) => a_Fam F
+  | (a_Const T) => a_Const T
+  | (a_Pi rho A R B) => a_Pi rho (open_tm_wrt_tm_rec k a5 A) R (open_tm_wrt_tm_rec (S k) a5 B)
+  | (a_Conv a g) => a_Conv (open_tm_wrt_tm_rec k a5 a) (open_co_wrt_tm_rec k a5 g)
+  | (a_CPi phi B) => a_CPi (open_constraint_wrt_tm_rec k a5 phi) (open_tm_wrt_tm_rec k a5 B)
+  | (a_CAbs phi b) => a_CAbs (open_constraint_wrt_tm_rec k a5 phi) (open_tm_wrt_tm_rec k a5 b)
+  | (a_UCAbs b) => a_UCAbs (open_tm_wrt_tm_rec k a5 b)
+  | (a_CApp a g) => a_CApp (open_tm_wrt_tm_rec k a5 a) (open_co_wrt_tm_rec k a5 g)
+  | a_Bullet => a_Bullet 
+  | (a_DataCon K) => a_DataCon K
+  | (a_Case a brs5) => a_Case (open_tm_wrt_tm_rec k a5 a) (open_brs_wrt_tm_rec k a5 brs5)
+end
+with open_constraint_wrt_tm_rec (k:nat) (a5:tm) (phi5:constraint) : constraint :=
+  match phi5 with
+  | (Eq a b A R) => Eq (open_tm_wrt_tm_rec k a5 a) (open_tm_wrt_tm_rec k a5 b) (open_tm_wrt_tm_rec k a5 A) R
+end.
+
+Definition open_sort_wrt_co_rec (k:nat) (g5:co) (sort5:sort) : sort :=
   match sort5 with
-  | (Tm A) => Tm (open_tm_wrt_tm_rec k a5 A)
-  | (Co phi) => Co (open_constraint_wrt_tm_rec k a5 phi)
-end.
-
-Definition open_sig_sort_wrt_tm_rec (k:nat) (a5:tm) (sig_sort5:sig_sort) : sig_sort :=
-  match sig_sort5 with
-  | (Cs A) => Cs (open_tm_wrt_tm_rec k a5 A)
-  | (Ax a A) => Ax (open_tm_wrt_tm_rec k a5 a) (open_tm_wrt_tm_rec k a5 A)
+  | (Tm A R) => Tm (open_tm_wrt_co_rec k g5 A) R
+  | (Co phi) => Co (open_constraint_wrt_co_rec k g5 phi)
 end.
 
 Definition open_sig_sort_wrt_co_rec (k:nat) (g5:co) (sig_sort5:sig_sort) : sig_sort :=
   match sig_sort5 with
   | (Cs A) => Cs (open_tm_wrt_co_rec k g5 A)
-  | (Ax a A) => Ax (open_tm_wrt_co_rec k g5 a) (open_tm_wrt_co_rec k g5 A)
+  | (Ax a A R) => Ax (open_tm_wrt_co_rec k g5 a) (open_tm_wrt_co_rec k g5 A) R
 end.
 
-Definition open_sort_wrt_co_rec (k:nat) (g5:co) (sort5:sort) : sort :=
+Definition open_sig_sort_wrt_tm_rec (k:nat) (a5:tm) (sig_sort5:sig_sort) : sig_sort :=
+  match sig_sort5 with
+  | (Cs A) => Cs (open_tm_wrt_tm_rec k a5 A)
+  | (Ax a A R) => Ax (open_tm_wrt_tm_rec k a5 a) (open_tm_wrt_tm_rec k a5 A) R
+end.
+
+Definition open_sort_wrt_tm_rec (k:nat) (a5:tm) (sort5:sort) : sort :=
   match sort5 with
-  | (Tm A) => Tm (open_tm_wrt_co_rec k g5 A)
-  | (Co phi) => Co (open_constraint_wrt_co_rec k g5 phi)
+  | (Tm A R) => Tm (open_tm_wrt_tm_rec k a5 A) R
+  | (Co phi) => Co (open_constraint_wrt_tm_rec k a5 phi)
 end.
-
-Definition open_sort_wrt_tm a5 sort5 := open_sort_wrt_tm_rec 0 sort5 a5.
-
-Definition open_sig_sort_wrt_tm a5 sig_sort5 := open_sig_sort_wrt_tm_rec 0 sig_sort5 a5.
-
-Definition open_brs_wrt_tm a5 brs_6 := open_brs_wrt_tm_rec 0 brs_6 a5.
-
-Definition open_constraint_wrt_tm a5 phi5 := open_constraint_wrt_tm_rec 0 phi5 a5.
-
-Definition open_tm_wrt_co g5 a5 := open_tm_wrt_co_rec 0 a5 g5.
-
-Definition open_co_wrt_tm a5 g_5 := open_co_wrt_tm_rec 0 g_5 a5.
 
 Definition open_brs_wrt_co g5 brs_6 := open_brs_wrt_co_rec 0 brs_6 g5.
 
-Definition open_sig_sort_wrt_co g5 sig_sort5 := open_sig_sort_wrt_co_rec 0 sig_sort5 g5.
+Definition open_tm_wrt_co g5 a5 := open_tm_wrt_co_rec 0 a5 g5.
+
+Definition open_brs_wrt_tm a5 brs_6 := open_brs_wrt_tm_rec 0 brs_6 a5.
 
 Definition open_sort_wrt_co g5 sort5 := open_sort_wrt_co_rec 0 sort5 g5.
 
-Definition open_tm_wrt_tm a5 a_6 := open_tm_wrt_tm_rec 0 a_6 a5.
+Definition open_sig_sort_wrt_co g5 sig_sort5 := open_sig_sort_wrt_co_rec 0 sig_sort5 g5.
+
+Definition open_co_wrt_co g_5 g__6 := open_co_wrt_co_rec 0 g__6 g_5.
+
+Definition open_sig_sort_wrt_tm a5 sig_sort5 := open_sig_sort_wrt_tm_rec 0 sig_sort5 a5.
 
 Definition open_constraint_wrt_co g5 phi5 := open_constraint_wrt_co_rec 0 phi5 g5.
 
-Definition open_co_wrt_co g_5 g__6 := open_co_wrt_co_rec 0 g__6 g_5.
+Definition open_constraint_wrt_tm a5 phi5 := open_constraint_wrt_tm_rec 0 phi5 a5.
+
+Definition open_co_wrt_tm a5 g_5 := open_co_wrt_tm_rec 0 g_5 a5.
+
+Definition open_sort_wrt_tm a5 sort5 := open_sort_wrt_tm_rec 0 sort5 a5.
+
+Definition open_tm_wrt_tm a5 a_6 := open_tm_wrt_tm_rec 0 a_6 a5.
 
 (** terms are locally-closed pre-terms *)
 (** definitions *)
 
-(* defns LC_constraint_co_brs_tm *)
-Inductive lc_constraint : constraint -> Prop :=    (* defn lc_constraint *)
- | lc_Eq : forall (a b A:tm),
-     (lc_tm a) ->
-     (lc_tm b) ->
-     (lc_tm A) ->
-     (lc_constraint (Eq a b A))
-with lc_co : co -> Prop :=    (* defn lc_co *)
+(* defns LC_co_brs_tm_constraint *)
+Inductive lc_co : co -> Prop :=    (* defn lc_co *)
  | lc_g_Triv : 
      (lc_co g_Triv)
  | lc_g_Var_f : forall (c:covar),
@@ -337,11 +335,11 @@ with lc_co : co -> Prop :=    (* defn lc_co *)
      (lc_co g1) ->
      (lc_co g2) ->
      (lc_co (g_Cast g1 g2))
- | lc_g_EqCong : forall (g1:co) (A:tm) (g2:co),
+ | lc_g_EqCong : forall (g1:co) (A:tm) (R:role) (g2:co),
      (lc_co g1) ->
      (lc_tm A) ->
      (lc_co g2) ->
-     (lc_co (g_EqCong g1 A g2))
+     (lc_co (g_EqCong g1 A R g2))
  | lc_g_IsoConv : forall (phi1 phi2:constraint) (g:co),
      (lc_constraint phi1) ->
      (lc_constraint phi2) ->
@@ -370,10 +368,10 @@ with lc_tm : tm -> Prop :=    (* defn lc_tm *)
      (lc_tm a_Star)
  | lc_a_Var_f : forall (x:tmvar),
      (lc_tm (a_Var_f x))
- | lc_a_Abs : forall (rho:relflag) (A b:tm),
+ | lc_a_Abs : forall (rho:relflag) (A:tm) (R:role) (b:tm),
      (lc_tm A) ->
       ( forall x , lc_tm  ( open_tm_wrt_tm b (a_Var_f x) )  )  ->
-     (lc_tm (a_Abs rho A b))
+     (lc_tm (a_Abs rho A R b))
  | lc_a_UAbs : forall (rho:relflag) (b:tm),
       ( forall x , lc_tm  ( open_tm_wrt_tm b (a_Var_f x) )  )  ->
      (lc_tm (a_UAbs rho b))
@@ -385,10 +383,10 @@ with lc_tm : tm -> Prop :=    (* defn lc_tm *)
      (lc_tm (a_Fam F))
  | lc_a_Const : forall (T:const),
      (lc_tm (a_Const T))
- | lc_a_Pi : forall (rho:relflag) (A B:tm),
+ | lc_a_Pi : forall (rho:relflag) (A:tm) (R:role) (B:tm),
      (lc_tm A) ->
       ( forall x , lc_tm  ( open_tm_wrt_tm B (a_Var_f x) )  )  ->
-     (lc_tm (a_Pi rho A B))
+     (lc_tm (a_Pi rho A R B))
  | lc_a_Conv : forall (a:tm) (g:co),
      (lc_tm a) ->
      (lc_co g) ->
@@ -415,13 +413,19 @@ with lc_tm : tm -> Prop :=    (* defn lc_tm *)
  | lc_a_Case : forall (a:tm) (brs5:brs),
      (lc_tm a) ->
      (lc_brs brs5) ->
-     (lc_tm (a_Case a brs5)).
+     (lc_tm (a_Case a brs5))
+with lc_constraint : constraint -> Prop :=    (* defn lc_constraint *)
+ | lc_Eq : forall (a b A:tm) (R:role),
+     (lc_tm a) ->
+     (lc_tm b) ->
+     (lc_tm A) ->
+     (lc_constraint (Eq a b A R)).
 
 (* defns LC_sort *)
 Inductive lc_sort : sort -> Prop :=    (* defn lc_sort *)
- | lc_Tm : forall (A:tm),
+ | lc_Tm : forall (A:tm) (R:role),
      (lc_tm A) ->
-     (lc_sort (Tm A))
+     (lc_sort (Tm A R))
  | lc_Co : forall (phi:constraint),
      (lc_constraint phi) ->
      (lc_sort (Co phi)).
@@ -431,10 +435,10 @@ Inductive lc_sig_sort : sig_sort -> Prop :=    (* defn lc_sig_sort *)
  | lc_Cs : forall (A:tm),
      (lc_tm A) ->
      (lc_sig_sort (Cs A))
- | lc_Ax : forall (a A:tm),
+ | lc_Ax : forall (a A:tm) (R:role),
      (lc_tm a) ->
      (lc_tm A) ->
-     (lc_sig_sort (Ax a A)).
+     (lc_sig_sort (Ax a A R)).
 (** free variables *)
 Fixpoint fv_tm_tm_co (g_5:co) : vars :=
   match g_5 with
@@ -458,7 +462,7 @@ Fixpoint fv_tm_tm_co (g_5:co) : vars :=
   | (g_CAppCong g g1 g2) => (fv_tm_tm_co g) \u (fv_tm_tm_co g1) \u (fv_tm_tm_co g2)
   | (g_CPiSnd g g1 g2) => (fv_tm_tm_co g) \u (fv_tm_tm_co g1) \u (fv_tm_tm_co g2)
   | (g_Cast g1 g2) => (fv_tm_tm_co g1) \u (fv_tm_tm_co g2)
-  | (g_EqCong g1 A g2) => (fv_tm_tm_co g1) \u (fv_tm_tm_tm A) \u (fv_tm_tm_co g2)
+  | (g_EqCong g1 A R g2) => (fv_tm_tm_co g1) \u (fv_tm_tm_tm A) \u (fv_tm_tm_co g2)
   | (g_IsoConv phi1 phi2 g) => (fv_tm_tm_constraint phi1) \u (fv_tm_tm_constraint phi2) \u (fv_tm_tm_co g)
   | (g_Eta a) => (fv_tm_tm_tm a)
   | (g_Left g g') => (fv_tm_tm_co g) \u (fv_tm_tm_co g')
@@ -474,12 +478,12 @@ with fv_tm_tm_tm (a5:tm) : vars :=
   | a_Star => {}
   | (a_Var_b nat) => {}
   | (a_Var_f x) => {{x}}
-  | (a_Abs rho A b) => (fv_tm_tm_tm A) \u (fv_tm_tm_tm b)
+  | (a_Abs rho A R b) => (fv_tm_tm_tm A) \u (fv_tm_tm_tm b)
   | (a_UAbs rho b) => (fv_tm_tm_tm b)
   | (a_App a rho b) => (fv_tm_tm_tm a) \u (fv_tm_tm_tm b)
   | (a_Fam F) => {}
   | (a_Const T) => {}
-  | (a_Pi rho A B) => (fv_tm_tm_tm A) \u (fv_tm_tm_tm B)
+  | (a_Pi rho A R B) => (fv_tm_tm_tm A) \u (fv_tm_tm_tm B)
   | (a_Conv a g) => (fv_tm_tm_tm a) \u (fv_tm_tm_co g)
   | (a_CPi phi B) => (fv_tm_tm_constraint phi) \u (fv_tm_tm_tm B)
   | (a_CAbs phi b) => (fv_tm_tm_constraint phi) \u (fv_tm_tm_tm b)
@@ -491,7 +495,7 @@ with fv_tm_tm_tm (a5:tm) : vars :=
 end
 with fv_tm_tm_constraint (phi5:constraint) : vars :=
   match phi5 with
-  | (Eq a b A) => (fv_tm_tm_tm a) \u (fv_tm_tm_tm b) \u (fv_tm_tm_tm A)
+  | (Eq a b A R) => (fv_tm_tm_tm a) \u (fv_tm_tm_tm b) \u (fv_tm_tm_tm A)
 end.
 
 Fixpoint fv_co_co_co (g_5:co) : vars :=
@@ -516,7 +520,7 @@ Fixpoint fv_co_co_co (g_5:co) : vars :=
   | (g_CAppCong g g1 g2) => (fv_co_co_co g) \u (fv_co_co_co g1) \u (fv_co_co_co g2)
   | (g_CPiSnd g g1 g2) => (fv_co_co_co g) \u (fv_co_co_co g1) \u (fv_co_co_co g2)
   | (g_Cast g1 g2) => (fv_co_co_co g1) \u (fv_co_co_co g2)
-  | (g_EqCong g1 A g2) => (fv_co_co_co g1) \u (fv_co_co_tm A) \u (fv_co_co_co g2)
+  | (g_EqCong g1 A R g2) => (fv_co_co_co g1) \u (fv_co_co_tm A) \u (fv_co_co_co g2)
   | (g_IsoConv phi1 phi2 g) => (fv_co_co_constraint phi1) \u (fv_co_co_constraint phi2) \u (fv_co_co_co g)
   | (g_Eta a) => (fv_co_co_tm a)
   | (g_Left g g') => (fv_co_co_co g) \u (fv_co_co_co g')
@@ -532,12 +536,12 @@ with fv_co_co_tm (a5:tm) : vars :=
   | a_Star => {}
   | (a_Var_b nat) => {}
   | (a_Var_f x) => {}
-  | (a_Abs rho A b) => (fv_co_co_tm A) \u (fv_co_co_tm b)
+  | (a_Abs rho A R b) => (fv_co_co_tm A) \u (fv_co_co_tm b)
   | (a_UAbs rho b) => (fv_co_co_tm b)
   | (a_App a rho b) => (fv_co_co_tm a) \u (fv_co_co_tm b)
   | (a_Fam F) => {}
   | (a_Const T) => {}
-  | (a_Pi rho A B) => (fv_co_co_tm A) \u (fv_co_co_tm B)
+  | (a_Pi rho A R B) => (fv_co_co_tm A) \u (fv_co_co_tm B)
   | (a_Conv a g) => (fv_co_co_tm a) \u (fv_co_co_co g)
   | (a_CPi phi B) => (fv_co_co_constraint phi) \u (fv_co_co_tm B)
   | (a_CAbs phi b) => (fv_co_co_constraint phi) \u (fv_co_co_tm b)
@@ -549,64 +553,35 @@ with fv_co_co_tm (a5:tm) : vars :=
 end
 with fv_co_co_constraint (phi5:constraint) : vars :=
   match phi5 with
-  | (Eq a b A) => (fv_co_co_tm a) \u (fv_co_co_tm b) \u (fv_co_co_tm A)
+  | (Eq a b A R) => (fv_co_co_tm a) \u (fv_co_co_tm b) \u (fv_co_co_tm A)
 end.
 
 Definition fv_tm_tm_sort (sort5:sort) : vars :=
   match sort5 with
-  | (Tm A) => (fv_tm_tm_tm A)
+  | (Tm A R) => (fv_tm_tm_tm A)
   | (Co phi) => (fv_tm_tm_constraint phi)
 end.
 
 Definition fv_co_co_sort (sort5:sort) : vars :=
   match sort5 with
-  | (Tm A) => (fv_co_co_tm A)
+  | (Tm A R) => (fv_co_co_tm A)
   | (Co phi) => (fv_co_co_constraint phi)
 end.
 
 Definition fv_tm_tm_sig_sort (sig_sort5:sig_sort) : vars :=
   match sig_sort5 with
   | (Cs A) => (fv_tm_tm_tm A)
-  | (Ax a A) => (fv_tm_tm_tm a) \u (fv_tm_tm_tm A)
+  | (Ax a A R) => (fv_tm_tm_tm a) \u (fv_tm_tm_tm A)
 end.
 
 Definition fv_co_co_sig_sort (sig_sort5:sig_sort) : vars :=
   match sig_sort5 with
   | (Cs A) => (fv_co_co_tm A)
-  | (Ax a A) => (fv_co_co_tm a) \u (fv_co_co_tm A)
+  | (Ax a A R) => (fv_co_co_tm a) \u (fv_co_co_tm A)
 end.
 
 (** substitutions *)
-Fixpoint tm_subst_tm_brs (a5:tm) (x5:tmvar) (brs_6:brs) {struct brs_6} : brs :=
-  match brs_6 with
-  | br_None => br_None 
-  | (br_One K a brs5) => br_One K (tm_subst_tm_tm a5 x5 a) (tm_subst_tm_brs a5 x5 brs5)
-end
-with tm_subst_tm_tm (a5:tm) (x5:tmvar) (a_6:tm) {struct a_6} : tm :=
-  match a_6 with
-  | a_Star => a_Star 
-  | (a_Var_b nat) => a_Var_b nat
-  | (a_Var_f x) => (if eq_var x x5 then a5 else (a_Var_f x))
-  | (a_Abs rho A b) => a_Abs rho (tm_subst_tm_tm a5 x5 A) (tm_subst_tm_tm a5 x5 b)
-  | (a_UAbs rho b) => a_UAbs rho (tm_subst_tm_tm a5 x5 b)
-  | (a_App a rho b) => a_App (tm_subst_tm_tm a5 x5 a) rho (tm_subst_tm_tm a5 x5 b)
-  | (a_Fam F) => a_Fam F
-  | (a_Const T) => a_Const T
-  | (a_Pi rho A B) => a_Pi rho (tm_subst_tm_tm a5 x5 A) (tm_subst_tm_tm a5 x5 B)
-  | (a_Conv a g) => a_Conv (tm_subst_tm_tm a5 x5 a) (tm_subst_tm_co a5 x5 g)
-  | (a_CPi phi B) => a_CPi (tm_subst_tm_constraint a5 x5 phi) (tm_subst_tm_tm a5 x5 B)
-  | (a_CAbs phi b) => a_CAbs (tm_subst_tm_constraint a5 x5 phi) (tm_subst_tm_tm a5 x5 b)
-  | (a_UCAbs b) => a_UCAbs (tm_subst_tm_tm a5 x5 b)
-  | (a_CApp a g) => a_CApp (tm_subst_tm_tm a5 x5 a) (tm_subst_tm_co a5 x5 g)
-  | a_Bullet => a_Bullet 
-  | (a_DataCon K) => a_DataCon K
-  | (a_Case a brs5) => a_Case (tm_subst_tm_tm a5 x5 a) (tm_subst_tm_brs a5 x5 brs5)
-end
-with tm_subst_tm_constraint (a5:tm) (x5:tmvar) (phi5:constraint) {struct phi5} : constraint :=
-  match phi5 with
-  | (Eq a b A) => Eq (tm_subst_tm_tm a5 x5 a) (tm_subst_tm_tm a5 x5 b) (tm_subst_tm_tm a5 x5 A)
-end
-with tm_subst_tm_co (a5:tm) (x5:tmvar) (g_5:co) {struct g_5} : co :=
+Fixpoint tm_subst_tm_co (a5:tm) (x5:tmvar) (g_5:co) {struct g_5} : co :=
   match g_5 with
   | g_Triv => g_Triv 
   | (g_Var_b nat) => g_Var_b nat
@@ -628,11 +603,40 @@ with tm_subst_tm_co (a5:tm) (x5:tmvar) (g_5:co) {struct g_5} : co :=
   | (g_CAppCong g g1 g2) => g_CAppCong (tm_subst_tm_co a5 x5 g) (tm_subst_tm_co a5 x5 g1) (tm_subst_tm_co a5 x5 g2)
   | (g_CPiSnd g g1 g2) => g_CPiSnd (tm_subst_tm_co a5 x5 g) (tm_subst_tm_co a5 x5 g1) (tm_subst_tm_co a5 x5 g2)
   | (g_Cast g1 g2) => g_Cast (tm_subst_tm_co a5 x5 g1) (tm_subst_tm_co a5 x5 g2)
-  | (g_EqCong g1 A g2) => g_EqCong (tm_subst_tm_co a5 x5 g1) (tm_subst_tm_tm a5 x5 A) (tm_subst_tm_co a5 x5 g2)
+  | (g_EqCong g1 A R g2) => g_EqCong (tm_subst_tm_co a5 x5 g1) (tm_subst_tm_tm a5 x5 A) R (tm_subst_tm_co a5 x5 g2)
   | (g_IsoConv phi1 phi2 g) => g_IsoConv (tm_subst_tm_constraint a5 x5 phi1) (tm_subst_tm_constraint a5 x5 phi2) (tm_subst_tm_co a5 x5 g)
   | (g_Eta a) => g_Eta (tm_subst_tm_tm a5 x5 a)
   | (g_Left g g') => g_Left (tm_subst_tm_co a5 x5 g) (tm_subst_tm_co a5 x5 g')
   | (g_Right g g') => g_Right (tm_subst_tm_co a5 x5 g) (tm_subst_tm_co a5 x5 g')
+end
+with tm_subst_tm_brs (a5:tm) (x5:tmvar) (brs_6:brs) {struct brs_6} : brs :=
+  match brs_6 with
+  | br_None => br_None 
+  | (br_One K a brs5) => br_One K (tm_subst_tm_tm a5 x5 a) (tm_subst_tm_brs a5 x5 brs5)
+end
+with tm_subst_tm_tm (a5:tm) (x5:tmvar) (a_6:tm) {struct a_6} : tm :=
+  match a_6 with
+  | a_Star => a_Star 
+  | (a_Var_b nat) => a_Var_b nat
+  | (a_Var_f x) => (if eq_var x x5 then a5 else (a_Var_f x))
+  | (a_Abs rho A R b) => a_Abs rho (tm_subst_tm_tm a5 x5 A) R (tm_subst_tm_tm a5 x5 b)
+  | (a_UAbs rho b) => a_UAbs rho (tm_subst_tm_tm a5 x5 b)
+  | (a_App a rho b) => a_App (tm_subst_tm_tm a5 x5 a) rho (tm_subst_tm_tm a5 x5 b)
+  | (a_Fam F) => a_Fam F
+  | (a_Const T) => a_Const T
+  | (a_Pi rho A R B) => a_Pi rho (tm_subst_tm_tm a5 x5 A) R (tm_subst_tm_tm a5 x5 B)
+  | (a_Conv a g) => a_Conv (tm_subst_tm_tm a5 x5 a) (tm_subst_tm_co a5 x5 g)
+  | (a_CPi phi B) => a_CPi (tm_subst_tm_constraint a5 x5 phi) (tm_subst_tm_tm a5 x5 B)
+  | (a_CAbs phi b) => a_CAbs (tm_subst_tm_constraint a5 x5 phi) (tm_subst_tm_tm a5 x5 b)
+  | (a_UCAbs b) => a_UCAbs (tm_subst_tm_tm a5 x5 b)
+  | (a_CApp a g) => a_CApp (tm_subst_tm_tm a5 x5 a) (tm_subst_tm_co a5 x5 g)
+  | a_Bullet => a_Bullet 
+  | (a_DataCon K) => a_DataCon K
+  | (a_Case a brs5) => a_Case (tm_subst_tm_tm a5 x5 a) (tm_subst_tm_brs a5 x5 brs5)
+end
+with tm_subst_tm_constraint (a5:tm) (x5:tmvar) (phi5:constraint) {struct phi5} : constraint :=
+  match phi5 with
+  | (Eq a b A R) => Eq (tm_subst_tm_tm a5 x5 a) (tm_subst_tm_tm a5 x5 b) (tm_subst_tm_tm a5 x5 A) R
 end.
 
 Fixpoint co_subst_co_co (g_5:co) (c5:covar) (g__6:co) {struct g__6} : co :=
@@ -657,7 +661,7 @@ Fixpoint co_subst_co_co (g_5:co) (c5:covar) (g__6:co) {struct g__6} : co :=
   | (g_CAppCong g g1 g2) => g_CAppCong (co_subst_co_co g_5 c5 g) (co_subst_co_co g_5 c5 g1) (co_subst_co_co g_5 c5 g2)
   | (g_CPiSnd g g1 g2) => g_CPiSnd (co_subst_co_co g_5 c5 g) (co_subst_co_co g_5 c5 g1) (co_subst_co_co g_5 c5 g2)
   | (g_Cast g1 g2) => g_Cast (co_subst_co_co g_5 c5 g1) (co_subst_co_co g_5 c5 g2)
-  | (g_EqCong g1 A g2) => g_EqCong (co_subst_co_co g_5 c5 g1) (co_subst_co_tm g_5 c5 A) (co_subst_co_co g_5 c5 g2)
+  | (g_EqCong g1 A R g2) => g_EqCong (co_subst_co_co g_5 c5 g1) (co_subst_co_tm g_5 c5 A) R (co_subst_co_co g_5 c5 g2)
   | (g_IsoConv phi1 phi2 g) => g_IsoConv (co_subst_co_constraint g_5 c5 phi1) (co_subst_co_constraint g_5 c5 phi2) (co_subst_co_co g_5 c5 g)
   | (g_Eta a) => g_Eta (co_subst_co_tm g_5 c5 a)
   | (g_Left g g') => g_Left (co_subst_co_co g_5 c5 g) (co_subst_co_co g_5 c5 g')
@@ -673,12 +677,12 @@ with co_subst_co_tm (g5:co) (c5:covar) (a5:tm) {struct a5} : tm :=
   | a_Star => a_Star 
   | (a_Var_b nat) => a_Var_b nat
   | (a_Var_f x) => a_Var_f x
-  | (a_Abs rho A b) => a_Abs rho (co_subst_co_tm g5 c5 A) (co_subst_co_tm g5 c5 b)
+  | (a_Abs rho A R b) => a_Abs rho (co_subst_co_tm g5 c5 A) R (co_subst_co_tm g5 c5 b)
   | (a_UAbs rho b) => a_UAbs rho (co_subst_co_tm g5 c5 b)
   | (a_App a rho b) => a_App (co_subst_co_tm g5 c5 a) rho (co_subst_co_tm g5 c5 b)
   | (a_Fam F) => a_Fam F
   | (a_Const T) => a_Const T
-  | (a_Pi rho A B) => a_Pi rho (co_subst_co_tm g5 c5 A) (co_subst_co_tm g5 c5 B)
+  | (a_Pi rho A R B) => a_Pi rho (co_subst_co_tm g5 c5 A) R (co_subst_co_tm g5 c5 B)
   | (a_Conv a g) => a_Conv (co_subst_co_tm g5 c5 a) (co_subst_co_co g5 c5 g)
   | (a_CPi phi B) => a_CPi (co_subst_co_constraint g5 c5 phi) (co_subst_co_tm g5 c5 B)
   | (a_CAbs phi b) => a_CAbs (co_subst_co_constraint g5 c5 phi) (co_subst_co_tm g5 c5 b)
@@ -690,31 +694,31 @@ with co_subst_co_tm (g5:co) (c5:covar) (a5:tm) {struct a5} : tm :=
 end
 with co_subst_co_constraint (g5:co) (c5:covar) (phi5:constraint) {struct phi5} : constraint :=
   match phi5 with
-  | (Eq a b A) => Eq (co_subst_co_tm g5 c5 a) (co_subst_co_tm g5 c5 b) (co_subst_co_tm g5 c5 A)
+  | (Eq a b A R) => Eq (co_subst_co_tm g5 c5 a) (co_subst_co_tm g5 c5 b) (co_subst_co_tm g5 c5 A) R
 end.
 
 Definition tm_subst_tm_sort (a5:tm) (x5:tmvar) (sort5:sort) : sort :=
   match sort5 with
-  | (Tm A) => Tm (tm_subst_tm_tm a5 x5 A)
+  | (Tm A R) => Tm (tm_subst_tm_tm a5 x5 A) R
   | (Co phi) => Co (tm_subst_tm_constraint a5 x5 phi)
 end.
 
 Definition co_subst_co_sort (g5:co) (c5:covar) (sort5:sort) : sort :=
   match sort5 with
-  | (Tm A) => Tm (co_subst_co_tm g5 c5 A)
+  | (Tm A R) => Tm (co_subst_co_tm g5 c5 A) R
   | (Co phi) => Co (co_subst_co_constraint g5 c5 phi)
 end.
 
 Definition tm_subst_tm_sig_sort (a5:tm) (x5:tmvar) (sig_sort5:sig_sort) : sig_sort :=
   match sig_sort5 with
   | (Cs A) => Cs (tm_subst_tm_tm a5 x5 A)
-  | (Ax a A) => Ax (tm_subst_tm_tm a5 x5 a) (tm_subst_tm_tm a5 x5 A)
+  | (Ax a A R) => Ax (tm_subst_tm_tm a5 x5 a) (tm_subst_tm_tm a5 x5 A) R
 end.
 
 Definition co_subst_co_sig_sort (g5:co) (c5:covar) (sig_sort5:sig_sort) : sig_sort :=
   match sig_sort5 with
   | (Cs A) => Cs (co_subst_co_tm g5 c5 A)
-  | (Ax a A) => Ax (co_subst_co_tm g5 c5 a) (co_subst_co_tm g5 c5 A)
+  | (Ax a A R) => Ax (co_subst_co_tm g5 c5 a) (co_subst_co_tm g5 c5 A) R
 end.
 
 Fixpoint erase_tm (a : tm) : tm :=
@@ -722,13 +726,13 @@ Fixpoint erase_tm (a : tm) : tm :=
    | a_Star    => a_Star
    | a_Var_b n => a_Var_b n
    | a_Var_f x => a_Var_f x
-   | a_Abs rho A b => a_UAbs rho (erase_tm b)
+   | a_Abs rho A R b => a_UAbs rho (erase_tm b)
    | a_UAbs rho b => a_UAbs rho (erase_tm b)
    | a_App a Rel b => a_App (erase_tm a) Rel (erase_tm b)
    | a_App a Irrel b => a_App (erase_tm a) Irrel a_Bullet
    | a_Const T => a_Const T
    | a_Fam F => a_Fam F
-   | a_Pi rho A B => a_Pi rho (erase_tm A) (erase_tm B)
+   | a_Pi rho A R B => a_Pi rho (erase_tm A) R (erase_tm B)
    | a_Conv a _ => erase_tm a
    | a_CPi phi B => a_CPi (erase_constraint phi) (erase_tm B)
    | a_CAbs phi b => a_UCAbs (erase_tm b)
@@ -745,12 +749,12 @@ with erase_brs (x : brs) : brs :=
    end
 with erase_constraint (phi : constraint) : constraint :=
    match phi with
-   | Eq A B A1 => Eq (erase_tm A) (erase_tm B) (erase_tm A1)
+   | Eq A B A1 R => Eq (erase_tm A) (erase_tm B) (erase_tm A1) R
    end.
 
 Definition erase_sort s :=
  match s with
- | Tm a => Tm (erase_tm a)
+ | Tm a R => Tm (erase_tm a) R
  | Co p => Co (erase_constraint p)
 end.
 
@@ -758,7 +762,7 @@ end.
 Definition erase_csort s :=
  match s with
  | Cs a   => Cs (erase_tm a)
- | Ax a A => Ax (erase_tm a) (erase_tm A)
+ | Ax a A R => Ax (erase_tm a) (erase_tm A) R
 end.
 
 Definition erase_context G := map erase_sort G.
@@ -771,24 +775,35 @@ Definition Fix : atom.
 Qed.
 
 Definition FixDef : tm :=
-  (a_Abs Irrel a_Star
-         (a_Abs Rel (a_Pi Rel (a_Var_b 0) (a_Var_b 1))
+  (a_Abs Irrel a_Star Rep
+         (a_Abs Rel (a_Pi Rel (a_Var_b 0) Rep (a_Var_b 1)) Rep
                 (a_App (a_Var_b 0) Rel
                        (a_App (a_App (a_Fam Fix) Irrel (a_Var_b 1)) Rel (a_Var_b 0))))).
 
 Definition FixTy : tm :=
-  a_Pi Irrel a_Star
-       (a_Pi Rel (a_Pi Rel (a_Var_b 0) (a_Var_b 1))
+  a_Pi Irrel a_Star Rep
+       (a_Pi Rel (a_Pi Rel (a_Var_b 0) Rep (a_Var_b 1)) Rep
              (a_Var_b 1)).
 
 
-Definition an_toplevel : sig := Fix ~ Ax FixDef FixTy.
+Definition an_toplevel : sig := Fix ~ Ax FixDef FixTy Nom.
 
 Definition toplevel : sig := erase_sig an_toplevel.
 
 
 
 (** definitions *)
+
+(* defns JSubRole *)
+Inductive SubRole : role -> role -> Prop :=    (* defn SubRole *)
+ | NomRep : 
+     SubRole Nom Rep
+ | Refl : forall (R:role),
+     SubRole R R
+ | Trans : forall (R1 R3 R2:role),
+     SubRole R1 R2 ->
+     SubRole R2 R3 ->
+     SubRole R1 R3.
 
 (* defns JValue *)
 Inductive CoercedValue : tm -> Prop :=    (* defn CoercedValue *)
@@ -802,28 +817,28 @@ Inductive CoercedValue : tm -> Prop :=    (* defn CoercedValue *)
 with Value : tm -> Prop :=    (* defn Value *)
  | Value_Star : 
      Value a_Star
- | Value_Pi : forall (rho:relflag) (A B:tm),
+ | Value_Pi : forall (rho:relflag) (A:tm) (R:role) (B:tm),
      lc_tm A ->
-     lc_tm (a_Pi rho A B) ->
-     Value (a_Pi rho A B)
+     lc_tm (a_Pi rho A R B) ->
+     Value (a_Pi rho A R B)
  | Value_CPi : forall (phi:constraint) (B:tm),
      lc_constraint phi ->
      lc_tm (a_CPi phi B) ->
      Value (a_CPi phi B)
- | Value_AbsRel : forall (A a:tm),
+ | Value_AbsRel : forall (A:tm) (R:role) (a:tm),
      lc_tm A ->
-     lc_tm (a_Abs Rel A a) ->
-     Value (a_Abs Rel A a)
+     lc_tm (a_Abs Rel A R a) ->
+     Value (a_Abs Rel A R a)
  | Value_UAbsRel : forall (a:tm),
      lc_tm (a_UAbs Rel a) ->
      Value (a_UAbs Rel a)
  | Value_UAbsIrrel : forall (L:vars) (a:tm),
       ( forall x , x \notin  L  -> Value  ( open_tm_wrt_tm a (a_Var_f x) )  )  ->
      Value (a_UAbs Irrel a)
- | Value_AbsIrrel : forall (L:vars) (A a:tm),
+ | Value_AbsIrrel : forall (L:vars) (A:tm) (R:role) (a:tm),
      lc_tm A ->
       ( forall x , x \notin  L  -> CoercedValue  ( open_tm_wrt_tm a (a_Var_f x) )  )  ->
-     Value (a_Abs Irrel A a)
+     Value (a_Abs Irrel A R a)
  | Value_CAbs : forall (phi:constraint) (a:tm),
      lc_constraint phi ->
      lc_tm (a_CAbs phi a) ->
@@ -834,10 +849,10 @@ with Value : tm -> Prop :=    (* defn Value *)
 with value_type : tm -> Prop :=    (* defn value_type *)
  | value_type_Star : 
      value_type a_Star
- | value_type_Pi : forall (rho:relflag) (A B:tm),
+ | value_type_Pi : forall (rho:relflag) (A:tm) (R:role) (B:tm),
      lc_tm A ->
-     lc_tm (a_Pi rho A B) ->
-     value_type (a_Pi rho A B)
+     lc_tm (a_Pi rho A R B) ->
+     value_type (a_Pi rho A R B)
  | value_type_CPi : forall (phi:constraint) (B:tm),
      lc_constraint phi ->
      lc_tm (a_CPi phi B) ->
@@ -847,12 +862,12 @@ with value_type : tm -> Prop :=    (* defn value_type *)
 Inductive consistent : tm -> tm -> Prop :=    (* defn consistent *)
  | consistent_a_Star : 
      consistent a_Star a_Star
- | consistent_a_Pi : forall (rho:relflag) (A1 B1 A2 B2:tm),
+ | consistent_a_Pi : forall (rho:relflag) (A1:tm) (R:role) (B1 A2 B2:tm),
      lc_tm A1 ->
-     lc_tm (a_Pi rho A1 B1) ->
+     lc_tm (a_Pi rho A1 R B1) ->
      lc_tm A2 ->
-     lc_tm (a_Pi rho A2 B2) ->
-     consistent  ( (a_Pi rho A1 B1) )   ( (a_Pi rho A2 B2) ) 
+     lc_tm (a_Pi rho A2 R B2) ->
+     consistent  ( (a_Pi rho A1 R B1) )   ( (a_Pi rho A2 R B2) ) 
  | consistent_a_CPi : forall (phi1:constraint) (A1:tm) (phi2:constraint) (A2:tm),
      lc_constraint phi1 ->
      lc_tm (a_CPi phi1 A1) ->
@@ -883,16 +898,16 @@ Inductive erased_tm : tm -> Prop :=    (* defn erased_tm *)
      erased_tm a ->
      erased_tm b ->
      erased_tm  ( (a_App a rho b) ) 
- | erased_a_Pi : forall (L:vars) (rho:relflag) (A B:tm),
+ | erased_a_Pi : forall (L:vars) (rho:relflag) (A:tm) (R:role) (B:tm),
      erased_tm A ->
       ( forall x , x \notin  L  -> erased_tm  ( open_tm_wrt_tm B (a_Var_f x) )  )  ->
-     erased_tm  ( (a_Pi rho A B) ) 
- | erased_a_CPi : forall (L:vars) (a b A B:tm),
+     erased_tm  ( (a_Pi rho A R B) ) 
+ | erased_a_CPi : forall (L:vars) (a b A:tm) (R:role) (B:tm),
      erased_tm a ->
      erased_tm b ->
      erased_tm A ->
       ( forall c , c \notin  L  -> erased_tm  ( open_tm_wrt_co B (g_Var_f c) )  )  ->
-     erased_tm  ( (a_CPi (Eq a b A) B) ) 
+     erased_tm  ( (a_CPi (Eq a b A R) B) ) 
  | erased_a_CAbs : forall (L:vars) (b:tm),
       ( forall c , c \notin  L  -> erased_tm  ( open_tm_wrt_co b (g_Var_f c) )  )  ->
      erased_tm  ( (a_UCAbs b) ) 
@@ -935,21 +950,21 @@ Inductive Par : context -> available_props -> tm -> tm -> Prop :=    (* defn Par
  | Par_Abs : forall (L:vars) (G:context) (D:available_props) (rho:relflag) (a a':tm),
       ( forall x , x \notin  L  -> Par G D  ( open_tm_wrt_tm a (a_Var_f x) )   ( open_tm_wrt_tm a' (a_Var_f x) )  )  ->
      Par G D (a_UAbs rho a) (a_UAbs rho a')
- | Par_Pi : forall (L:vars) (G:context) (D:available_props) (rho:relflag) (A B A' B':tm),
+ | Par_Pi : forall (L:vars) (G:context) (D:available_props) (rho:relflag) (A:tm) (R:role) (B A' B':tm),
      Par G D A A' ->
       ( forall x , x \notin  L  -> Par G D  ( open_tm_wrt_tm B (a_Var_f x) )   ( open_tm_wrt_tm B' (a_Var_f x) )  )  ->
-     Par G D (a_Pi rho A B) (a_Pi rho A' B')
+     Par G D (a_Pi rho A R B) (a_Pi rho A' R B')
  | Par_CAbs : forall (L:vars) (G:context) (D:available_props) (a a':tm),
       ( forall c , c \notin  L  -> Par G D  ( open_tm_wrt_co a (g_Var_f c) )   ( open_tm_wrt_co a' (g_Var_f c) )  )  ->
      Par G D (a_UCAbs a) (a_UCAbs a')
- | Par_CPi : forall (L:vars) (G:context) (D:available_props) (A B A1 a A' B' A1' a':tm),
+ | Par_CPi : forall (L:vars) (G:context) (D:available_props) (A B A1:tm) (R:role) (a A' B' A1' a':tm),
      Par G D A A' ->
      Par G D B B' ->
       ( forall c , c \notin  L  -> Par G D  ( open_tm_wrt_co a (g_Var_f c) )   ( open_tm_wrt_co a' (g_Var_f c) )  )  ->
      Par G D A1 A1' ->
-     Par G D (a_CPi (Eq A B A1) a) (a_CPi (Eq A' B' A1') a')
- | Par_Axiom : forall (G:context) (D:available_props) (F:tyfam) (a A:tm),
-      binds  F  (Ax  a A )   toplevel   ->
+     Par G D (a_CPi (Eq A B A1 R) a) (a_CPi (Eq A' B' A1' R) a')
+ | Par_Axiom : forall (G:context) (D:available_props) (F:tyfam) (a A:tm) (R:role),
+      binds  F  (Ax  a A R )   toplevel   ->
      Par G D (a_Fam F) a
 with MultiPar : context -> available_props -> tm -> tm -> Prop :=    (* defn MultiPar *)
  | MP_Refl : forall (G:context) (D:available_props) (a:tm),
@@ -974,8 +989,8 @@ Inductive Beta : tm -> tm -> Prop :=    (* defn Beta *)
  | Beta_CAppCAbs : forall (a':tm),
      lc_tm (a_UCAbs a') ->
      Beta (a_CApp  ( (a_UCAbs a') )  g_Triv)  (open_tm_wrt_co  a'   g_Triv ) 
- | Beta_Axiom : forall (F:tyfam) (a A:tm),
-      binds  F  (Ax  a A )   toplevel   ->
+ | Beta_Axiom : forall (F:tyfam) (a A:tm) (R:role),
+      binds  F  (Ax  a A R )   toplevel   ->
      Beta (a_Fam F) a
 with reduction_in_one : tm -> tm -> Prop :=    (* defn reduction_in_one *)
  | E_AbsTerm : forall (L:vars) (a a':tm),
@@ -995,8 +1010,8 @@ with reduction_in_one : tm -> tm -> Prop :=    (* defn reduction_in_one *)
  | E_CAppCAbs : forall (b:tm),
      lc_tm (a_UCAbs b) ->
      reduction_in_one (a_CApp  ( (a_UCAbs b) )  g_Triv)  (open_tm_wrt_co  b   g_Triv ) 
- | E_Axiom : forall (F:tyfam) (a A:tm),
-      binds  F  (Ax  a A )   toplevel   ->
+ | E_Axiom : forall (F:tyfam) (a A:tm) (R:role),
+      binds  F  (Ax  a A R )   toplevel   ->
      reduction_in_one (a_Fam F) a
 with reduction : tm -> tm -> Prop :=    (* defn reduction *)
  | Equal : forall (a:tm),
@@ -1009,159 +1024,176 @@ with reduction : tm -> tm -> Prop :=    (* defn reduction *)
 
 (* defns Jett *)
 Inductive PropWff : context -> constraint -> Prop :=    (* defn PropWff *)
- | E_Wff : forall (G:context) (a b A:tm),
-     Typing G a A ->
-     Typing G b A ->
-      ( Typing G A a_Star )  ->
-     PropWff G (Eq a b A)
-with Typing : context -> tm -> tm -> Prop :=    (* defn Typing *)
- | E_Star : forall (G:context),
+ | E_Wff : forall (G:context) (a b A:tm) (R:role),
+     Typing G a A R ->
+     Typing G b A R ->
+      ( Typing G A a_Star R )  ->
+     PropWff G (Eq a b A R)
+with Typing : context -> tm -> tm -> role -> Prop :=    (* defn Typing *)
+ | E_SubRole : forall (G:context) (a A:tm) (R2 R1:role),
+     SubRole R1 R2 ->
+     Typing G a A R1 ->
+     Typing G a A R2
+ | E_Star : forall (G:context) (R:role),
      Ctx G ->
-     Typing G a_Star a_Star
- | E_Var : forall (G:context) (x:tmvar) (A:tm),
+     Typing G a_Star a_Star R
+ | E_Var : forall (G:context) (x:tmvar) (A:tm) (R:role),
      Ctx G ->
-      binds  x  (Tm  A )  G  ->
-     Typing G (a_Var_f x) A
- | E_Pi : forall (L:vars) (G:context) (rho:relflag) (A B:tm),
-      ( forall x , x \notin  L  -> Typing  (( x ~ Tm  A ) ++  G )   ( open_tm_wrt_tm B (a_Var_f x) )  a_Star )  ->
-      ( Typing G A a_Star )  ->
-     Typing G (a_Pi rho A B) a_Star
- | E_Abs : forall (L:vars) (G:context) (rho:relflag) (a A B:tm),
-      ( forall x , x \notin  L  -> Typing  (( x ~ Tm  A ) ++  G )   ( open_tm_wrt_tm a (a_Var_f x) )   ( open_tm_wrt_tm B (a_Var_f x) )  )  ->
-      ( Typing G A a_Star )  ->
+      binds  x  (Tm  A R )  G  ->
+     Typing G (a_Var_f x) A R
+ | E_Pi : forall (L:vars) (G:context) (rho:relflag) (A:tm) (R:role) (B:tm),
+      ( forall x , x \notin  L  -> Typing  (( x ~ Tm  A R ) ++  G )   ( open_tm_wrt_tm B (a_Var_f x) )  a_Star R )  ->
+      ( Typing G A a_Star R )  ->
+     Typing G (a_Pi rho A R B) a_Star R
+ | E_Abs : forall (L:vars) (G:context) (rho:relflag) (a A:tm) (R:role) (B:tm) (R':role),
+      ( forall x , x \notin  L  -> Typing  (( x ~ Tm  A R ) ++  G )   ( open_tm_wrt_tm a (a_Var_f x) )   ( open_tm_wrt_tm B (a_Var_f x) )  R' )  ->
+      ( Typing G A a_Star R )  ->
       ( forall x , x \notin  L  -> RhoCheck rho x  ( open_tm_wrt_tm a (a_Var_f x) )  )  ->
-     Typing G (a_UAbs rho a) (a_Pi rho A B)
- | E_App : forall (G:context) (b a B A:tm),
-     Typing G b (a_Pi Rel A B) ->
-     Typing G a A ->
-     Typing G (a_App b Rel a)  (open_tm_wrt_tm  B   a ) 
- | E_IApp : forall (G:context) (b B a A:tm),
-     Typing G b (a_Pi Irrel A B) ->
-     Typing G a A ->
-     Typing G (a_App b Irrel a_Bullet)  (open_tm_wrt_tm  B   a ) 
- | E_Conv : forall (G:context) (a B A:tm),
-     Typing G a A ->
-     DefEq G  (dom  G )  A B a_Star ->
-      ( Typing G B a_Star )  ->
-     Typing G a B
- | E_CPi : forall (L:vars) (G:context) (phi:constraint) (B:tm),
-      ( forall c , c \notin  L  -> Typing  (( c ~ Co  phi ) ++  G )   ( open_tm_wrt_co B (g_Var_f c) )  a_Star )  ->
+     SubRole R R' ->
+     Typing G (a_UAbs rho a)  ( (a_Pi rho A R B) )  R'
+ | E_App : forall (G:context) (b a B:tm) (R':role) (A:tm) (R:role),
+     Typing G b (a_Pi Rel A R B) R' ->
+     Typing G a A R ->
+     Typing G (a_App b Rel a)  (open_tm_wrt_tm  B   a )  R'
+ | E_IApp : forall (G:context) (b B a:tm) (R':role) (A:tm) (R:role),
+     Typing G b (a_Pi Irrel A R B) R' ->
+     Typing G a A R ->
+     Typing G (a_App b Irrel a_Bullet)  (open_tm_wrt_tm  B   a )  R'
+ | E_Conv : forall (G:context) (a B:tm) (R:role) (A:tm),
+     Typing G a A R ->
+     DefEq G  (dom  G )  A B a_Star R ->
+      ( Typing G B a_Star R )  ->
+     Typing G a B R
+ | E_CPi : forall (L:vars) (G:context) (phi:constraint) (B:tm) (R:role),
+      ( forall c , c \notin  L  -> Typing  (( c ~ Co  phi ) ++  G )   ( open_tm_wrt_co B (g_Var_f c) )  a_Star R )  ->
       ( PropWff G phi )  ->
-     Typing G (a_CPi phi B) a_Star
- | E_CAbs : forall (L:vars) (G:context) (a:tm) (phi:constraint) (B:tm),
-      ( forall c , c \notin  L  -> Typing  (( c ~ Co  phi ) ++  G )   ( open_tm_wrt_co a (g_Var_f c) )   ( open_tm_wrt_co B (g_Var_f c) )  )  ->
+     Typing G (a_CPi phi B) a_Star R
+ | E_CAbs : forall (L:vars) (G:context) (a:tm) (phi:constraint) (B:tm) (R:role),
+      ( forall c , c \notin  L  -> Typing  (( c ~ Co  phi ) ++  G )   ( open_tm_wrt_co a (g_Var_f c) )   ( open_tm_wrt_co B (g_Var_f c) )  R )  ->
       ( PropWff G phi )  ->
-     Typing G (a_UCAbs a) (a_CPi phi B)
- | E_CApp : forall (G:context) (a1 B1 a b A:tm),
-     Typing G a1 (a_CPi  ( (Eq a b A) )  B1) ->
-     DefEq G  (dom  G )  a b A ->
-     Typing G (a_CApp a1 g_Triv)  (open_tm_wrt_co  B1   g_Triv ) 
- | E_Fam : forall (G:context) (F:tyfam) (A a:tm),
+     Typing G (a_UCAbs a) (a_CPi phi B) R
+ | E_CApp : forall (G:context) (a1 B1:tm) (R':role) (a b A:tm) (R:role),
+     Typing G a1 (a_CPi  ( (Eq a b A R) )  B1) R' ->
+     DefEq G  (dom  G )  a b A R ->
+     Typing G (a_CApp a1 g_Triv)  (open_tm_wrt_co  B1   g_Triv )  R'
+ | E_Fam : forall (G:context) (F:tyfam) (A:tm) (R:role) (a:tm),
      Ctx G ->
-      binds  F  (Ax  a A )   toplevel   ->
-      ( Typing  nil  A a_Star )  ->
-     Typing G (a_Fam F) A
+      binds  F  (Ax  a A R )   toplevel   ->
+      ( Typing  nil  A a_Star R )  ->
+     Typing G (a_Fam F) A R
 with Iso : context -> available_props -> constraint -> constraint -> Prop :=    (* defn Iso *)
- | E_PropCong : forall (G:context) (D:available_props) (A1 B1 A A2 B2:tm),
-     DefEq G D A1 A2 A ->
-     DefEq G D B1 B2 A ->
-     Iso G D (Eq A1 B1 A) (Eq A2 B2 A)
- | E_IsoConv : forall (G:context) (D:available_props) (A1 A2 A B:tm),
-     DefEq G D A B a_Star ->
-     PropWff G (Eq A1 A2 A) ->
-     PropWff G (Eq A1 A2 B) ->
-     Iso G D (Eq A1 A2 A) (Eq A1 A2 B)
- | E_CPiFst : forall (G:context) (D:available_props) (phi1 phi2:constraint) (B1 B2:tm),
-     DefEq G D (a_CPi phi1 B1) (a_CPi phi2 B2) a_Star ->
+ | E_PropCong : forall (G:context) (D:available_props) (A1 B1 A:tm) (R:role) (A2 B2:tm),
+     DefEq G D A1 A2 A R ->
+     DefEq G D B1 B2 A R ->
+     Iso G D (Eq A1 B1 A R) (Eq A2 B2 A R)
+ | E_IsoConv : forall (G:context) (D:available_props) (A1 A2 A:tm) (R:role) (B:tm),
+     DefEq G D A B a_Star R ->
+     PropWff G (Eq A1 A2 A R) ->
+     PropWff G (Eq A1 A2 B R) ->
+     Iso G D (Eq A1 A2 A R) (Eq A1 A2 B R)
+ | E_CPiFst : forall (G:context) (D:available_props) (phi1 phi2:constraint) (B1 B2:tm) (R:role),
+     DefEq G D (a_CPi phi1 B1) (a_CPi phi2 B2) a_Star R ->
      Iso G D phi1 phi2
-with DefEq : context -> available_props -> tm -> tm -> tm -> Prop :=    (* defn DefEq *)
- | E_Assn : forall (G:context) (D:available_props) (a b A:tm) (c:covar),
+with DefEq : context -> available_props -> tm -> tm -> tm -> role -> Prop :=    (* defn DefEq *)
+ | E_Assn : forall (G:context) (D:available_props) (a b A:tm) (R:role) (c:covar),
      Ctx G ->
-      binds  c  (Co   ( (Eq a b A) )  )  G  ->
+      binds  c  (Co   ( (Eq a b A R) )  )  G  ->
       AtomSetImpl.In  c   D  ->
-     DefEq G D a b A
- | E_Refl : forall (G:context) (D:available_props) (a A:tm),
-     Typing G a A ->
-     DefEq G D a a A
- | E_Sym : forall (G:context) (D:available_props) (a b A:tm),
-     DefEq G D b a A ->
-     DefEq G D a b A
- | E_Trans : forall (G:context) (D:available_props) (a b A a1:tm),
-     DefEq G D a a1 A ->
-     DefEq G D a1 b A ->
-     DefEq G D a b A
- | E_Beta : forall (G:context) (D:available_props) (a1 a2 B:tm),
-     Typing G a1 B ->
-      ( Typing G a2 B )  ->
+     DefEq G D a b A R
+ | E_Refl : forall (G:context) (D:available_props) (a A:tm) (R:role),
+     Typing G a A R ->
+     DefEq G D a a A R
+ | E_Sym : forall (G:context) (D:available_props) (a b A:tm) (R:role),
+     DefEq G D b a A R ->
+     DefEq G D a b A R
+ | E_Trans : forall (G:context) (D:available_props) (a b A:tm) (R:role) (a1:tm),
+     DefEq G D a a1 A R ->
+     DefEq G D a1 b A R ->
+     DefEq G D a b A R
+ | E_Sub : forall (G:context) (D:available_props) (a b A:tm) (R2 R1:role),
+     DefEq G D a b A R1 ->
+     SubRole R1 R2 ->
+     DefEq G D a b A R2
+ | E_Beta : forall (G:context) (D:available_props) (a1 a2 B:tm) (R:role),
+     Typing G a1 B R ->
+      ( Typing G a2 B R )  ->
      Beta a1 a2 ->
-     DefEq G D a1 a2 B
- | E_PiCong : forall (L:vars) (G:context) (D:available_props) (rho:relflag) (A1 B1 A2 B2:tm),
-     DefEq G D A1 A2 a_Star ->
-      ( forall x , x \notin  L  -> DefEq  (( x ~ Tm  A1 ) ++  G )  D  ( open_tm_wrt_tm B1 (a_Var_f x) )   ( open_tm_wrt_tm B2 (a_Var_f x) )  a_Star )  ->
-      ( Typing G A1 a_Star )  ->
-      ( Typing G (a_Pi rho A1 B1) a_Star )  ->
-      ( Typing G (a_Pi rho A2 B2) a_Star )  ->
-     DefEq G D  ( (a_Pi rho A1 B1) )   ( (a_Pi rho A2 B2) )  a_Star
- | E_AbsCong : forall (L:vars) (G:context) (D:available_props) (rho:relflag) (b1 b2 A1 B:tm),
-      ( forall x , x \notin  L  -> DefEq  (( x ~ Tm  A1 ) ++  G )  D  ( open_tm_wrt_tm b1 (a_Var_f x) )   ( open_tm_wrt_tm b2 (a_Var_f x) )   ( open_tm_wrt_tm B (a_Var_f x) )  )  ->
-      ( Typing G A1 a_Star )  ->
+     DefEq G D a1 a2 B R
+ | E_PiCong : forall (L:vars) (G:context) (D:available_props) (rho:relflag) (A1:tm) (R:role) (B1 A2 B2:tm),
+     DefEq G D A1 A2 a_Star R ->
+      ( forall x , x \notin  L  -> DefEq  (( x ~ Tm  A1 R ) ++  G )  D  ( open_tm_wrt_tm B1 (a_Var_f x) )   ( open_tm_wrt_tm B2 (a_Var_f x) )  a_Star R )  ->
+      ( Typing G A1 a_Star R )  ->
+      ( Typing G (a_Pi rho A1 R B1) a_Star R )  ->
+      ( Typing G (a_Pi rho A2 R B2) a_Star R )  ->
+     DefEq G D  ( (a_Pi rho A1 R B1) )   ( (a_Pi rho A2 R B2) )  a_Star R
+ | E_AbsCong : forall (L:vars) (G:context) (D:available_props) (rho:relflag) (b1 b2 A1:tm) (R:role) (B:tm) (R':role),
+      ( forall x , x \notin  L  -> DefEq  (( x ~ Tm  A1 R ) ++  G )  D  ( open_tm_wrt_tm b1 (a_Var_f x) )   ( open_tm_wrt_tm b2 (a_Var_f x) )   ( open_tm_wrt_tm B (a_Var_f x) )  R' )  ->
+      ( Typing G A1 a_Star R )  ->
+      ( SubRole R R' )  ->
       ( forall x , x \notin  L  -> RhoCheck rho x  ( open_tm_wrt_tm b1 (a_Var_f x) )  )  ->
       ( forall x , x \notin  L  -> RhoCheck rho x  ( open_tm_wrt_tm b2 (a_Var_f x) )  )  ->
-     DefEq G D  ( (a_UAbs rho b1) )   ( (a_UAbs rho b2) )  (a_Pi rho A1 B)
- | E_AppCong : forall (G:context) (D:available_props) (a1 a2 b1 b2 B A:tm),
-     DefEq G D a1 b1 (a_Pi Rel A B) ->
-     DefEq G D a2 b2 A ->
-     DefEq G D (a_App a1 Rel a2) (a_App b1 Rel b2)  (open_tm_wrt_tm  B   a2 ) 
- | E_IAppCong : forall (G:context) (D:available_props) (a1 b1 B a A:tm),
-     DefEq G D a1 b1 (a_Pi Irrel A B) ->
-     Typing G a A ->
-     DefEq G D (a_App a1 Irrel a_Bullet) (a_App b1 Irrel a_Bullet)  (open_tm_wrt_tm  B   a ) 
- | E_PiFst : forall (G:context) (D:available_props) (A1 A2:tm) (rho:relflag) (B1 B2:tm),
-     DefEq G D (a_Pi rho A1 B1) (a_Pi rho A2 B2) a_Star ->
-     DefEq G D A1 A2 a_Star
- | E_PiSnd : forall (G:context) (D:available_props) (B1 a1 B2 a2:tm) (rho:relflag) (A1 A2:tm),
-     DefEq G D (a_Pi rho A1 B1) (a_Pi rho A2 B2) a_Star ->
-     DefEq G D a1 a2 A1 ->
-     DefEq G D  (open_tm_wrt_tm  B1   a1 )   (open_tm_wrt_tm  B2   a2 )  a_Star
- | E_CPiCong : forall (L:vars) (G:context) (D:available_props) (phi1:constraint) (A:tm) (phi2:constraint) (B:tm),
+     DefEq G D  ( (a_UAbs rho b1) )   ( (a_UAbs rho b2) )   ( (a_Pi rho A1 R B) )  R'
+ | E_AppCong : forall (G:context) (D:available_props) (a1 a2 b1 b2 B:tm) (R':role) (A:tm) (R:role),
+     DefEq G D a1 b1  ( (a_Pi Rel A R B) )  R' ->
+     DefEq G D a2 b2 A R ->
+     DefEq G D (a_App a1 Rel a2) (a_App b1 Rel b2)  (  (open_tm_wrt_tm  B   a2 )  )  R'
+ | E_IAppCong : forall (G:context) (D:available_props) (a1 b1 B a:tm) (R':role) (A:tm) (R:role),
+     DefEq G D a1 b1  ( (a_Pi Irrel A R B) )  R' ->
+     Typing G a A R ->
+     DefEq G D (a_App a1 Irrel a_Bullet) (a_App b1 Irrel a_Bullet)  (  (open_tm_wrt_tm  B   a )  )  R'
+ | E_PiFst : forall (G:context) (D:available_props) (A1 A2:tm) (R3:role) (rho:relflag) (R1:role) (B1:tm) (R2:role) (B2:tm) (R':role),
+     DefEq G D (a_Pi rho A1 R1 B1) (a_Pi rho A2 R2 B2) a_Star R' ->
+     SubRole R3 R1 ->
+     SubRole R3 R2 ->
+     DefEq G D A1 A2 a_Star R3
+ | E_PiSnd : forall (G:context) (D:available_props) (B1 a1 B2 a2:tm) (R':role) (rho:relflag) (A1:tm) (R1:role) (A2:tm) (R2 R:role),
+     DefEq G D (a_Pi rho A1 R1 B1) (a_Pi rho A2 R2 B2) a_Star R' ->
+     DefEq G D a1 a2 A1 R ->
+     SubRole R R1 ->
+     SubRole R R2 ->
+     DefEq G D  (open_tm_wrt_tm  B1   a1 )   (open_tm_wrt_tm  B2   a2 )  a_Star R'
+ | E_CPiCong : forall (L:vars) (G:context) (D:available_props) (phi1:constraint) (A:tm) (phi2:constraint) (B:tm) (R:role),
      Iso G D phi1 phi2 ->
-      ( forall c , c \notin  L  -> DefEq  (( c ~ Co  phi1 ) ++  G )  D  ( open_tm_wrt_co A (g_Var_f c) )   ( open_tm_wrt_co B (g_Var_f c) )  a_Star )  ->
+      ( forall c , c \notin  L  -> DefEq  (( c ~ Co  phi1 ) ++  G )  D  ( open_tm_wrt_co A (g_Var_f c) )   ( open_tm_wrt_co B (g_Var_f c) )  a_Star R )  ->
       ( PropWff G phi1 )  ->
-      ( Typing G (a_CPi phi1 A) a_Star )  ->
-      ( Typing G (a_CPi phi2 B) a_Star )  ->
-     DefEq G D (a_CPi phi1 A) (a_CPi phi2 B) a_Star
- | E_CAbsCong : forall (L:vars) (G:context) (D:available_props) (a b:tm) (phi1:constraint) (B:tm),
-      ( forall c , c \notin  L  -> DefEq  (( c ~ Co  phi1 ) ++  G )  D  ( open_tm_wrt_co a (g_Var_f c) )   ( open_tm_wrt_co b (g_Var_f c) )   ( open_tm_wrt_co B (g_Var_f c) )  )  ->
+      ( Typing G (a_CPi phi1 A) a_Star R )  ->
+      ( Typing G (a_CPi phi2 B) a_Star R )  ->
+     DefEq G D (a_CPi phi1 A) (a_CPi phi2 B) a_Star R
+ | E_CAbsCong : forall (L:vars) (G:context) (D:available_props) (a b:tm) (phi1:constraint) (B:tm) (R:role),
+      ( forall c , c \notin  L  -> DefEq  (( c ~ Co  phi1 ) ++  G )  D  ( open_tm_wrt_co a (g_Var_f c) )   ( open_tm_wrt_co b (g_Var_f c) )   ( open_tm_wrt_co B (g_Var_f c) )  R )  ->
       ( PropWff G phi1 )  ->
-     DefEq G D  ( (a_UCAbs a) )   ( (a_UCAbs b) )  (a_CPi phi1 B)
- | E_CAppCong : forall (G:context) (D:available_props) (a1 b1 B a b A:tm),
-     DefEq G D a1 b1 (a_CPi  ( (Eq a b A) )  B) ->
-     DefEq G  (dom  G )  a b A ->
-     DefEq G D (a_CApp a1 g_Triv) (a_CApp b1 g_Triv)  (open_tm_wrt_co  B   g_Triv ) 
- | E_CPiSnd : forall (G:context) (D:available_props) (B1 B2 a1 a2 A a1' a2' A':tm),
-     DefEq G D (a_CPi  ( (Eq a1 a2 A) )  B1) (a_CPi  ( (Eq a1' a2' A') )  B2) a_Star ->
-     DefEq G  (dom  G )  a1 a2 A ->
-     DefEq G  (dom  G )  a1' a2' A' ->
-     DefEq G D  (open_tm_wrt_co  B1   g_Triv )   (open_tm_wrt_co  B2   g_Triv )  a_Star
- | E_Cast : forall (G:context) (D:available_props) (a' b' A' a b A:tm),
-     DefEq G D a b A ->
-     Iso G D (Eq a b A) (Eq a' b' A') ->
-     DefEq G D a' b' A'
- | E_EqConv : forall (G:context) (D:available_props) (a b B A:tm),
-     DefEq G D a b A ->
-     DefEq G  (dom  G )  A B a_Star ->
-     DefEq G D a b B
- | E_IsoSnd : forall (G:context) (D:available_props) (A A' a b a' b':tm),
-     Iso G D (Eq a b A) (Eq a' b' A') ->
-     DefEq G D A A' a_Star
+     DefEq G D  ( (a_UCAbs a) )   ( (a_UCAbs b) )  (a_CPi phi1 B) R
+ | E_CAppCong : forall (G:context) (D:available_props) (a1 b1 B:tm) (R':role) (a b A:tm) (R:role),
+     DefEq G D a1 b1  ( (a_CPi  ( (Eq a b A R) )  B) )  R' ->
+     DefEq G  (dom  G )  a b A R ->
+     DefEq G D (a_CApp a1 g_Triv) (a_CApp b1 g_Triv)  (  (open_tm_wrt_co  B   g_Triv )  )  R'
+ | E_CPiSnd : forall (G:context) (D:available_props) (B1 B2:tm) (R0:role) (a1 a2 A:tm) (R:role) (a1' a2' A':tm) (R':role),
+     DefEq G D (a_CPi  ( (Eq a1 a2 A R) )  B1) (a_CPi  ( (Eq a1' a2' A' R') )  B2) a_Star R0 ->
+     DefEq G  (dom  G )  a1 a2 A R ->
+     DefEq G  (dom  G )  a1' a2' A' R' ->
+     DefEq G D  (open_tm_wrt_co  B1   g_Triv )   (open_tm_wrt_co  B2   g_Triv )  a_Star R0
+ | E_Cast : forall (G:context) (D:available_props) (a' b' A':tm) (R':role) (a b A:tm) (R:role),
+     DefEq G D a b A R ->
+     Iso G D (Eq a b A R) (Eq a' b' A' R') ->
+     DefEq G D a' b' A' R'
+ | E_EqConv : forall (G:context) (D:available_props) (a b B:tm) (R2:role) (A:tm) (R1:role),
+     DefEq G D a b A R1 ->
+     DefEq G  (dom  G )  A B a_Star R2 ->
+      ( SubRole R1 R2 )  ->
+     DefEq G D a b B R2
+ | E_IsoSnd : forall (G:context) (D:available_props) (A A':tm) (R0:role) (a b:tm) (R:role) (a' b':tm) (R':role),
+     Iso G D (Eq a b A R) (Eq a' b' A' R') ->
+     SubRole R R0 ->
+     SubRole R' R0 ->
+     DefEq G D A A' a_Star R0
 with Ctx : context -> Prop :=    (* defn Ctx *)
  | E_Empty : 
      Ctx  nil 
- | E_ConsTm : forall (G:context) (x:tmvar) (A:tm),
+ | E_ConsTm : forall (G:context) (x:tmvar) (A:tm) (R:role),
      Ctx G ->
-     Typing G A a_Star ->
+     Typing G A a_Star R ->
       ~ AtomSetImpl.In  x  (dom  G )  ->
-     Ctx  (( x ~ Tm  A ) ++  G ) 
+     Ctx  (( x ~ Tm  A R ) ++  G ) 
  | E_ConsCo : forall (G:context) (c:covar) (phi:constraint),
      Ctx G ->
      PropWff G phi ->
@@ -1172,196 +1204,206 @@ with Ctx : context -> Prop :=    (* defn Ctx *)
 Inductive Sig : sig -> Prop :=    (* defn Sig *)
  | Sig_Empty : 
      Sig  nil 
- | Sig_ConsAx : forall (S:sig) (F:tyfam) (a A:tm),
+ | Sig_ConsAx : forall (S:sig) (F:tyfam) (a A:tm) (R' R:role),
      Sig S ->
-     Typing  nil  A a_Star ->
-     Typing  nil  a A ->
+     Typing  nil  A a_Star R ->
+     Typing  nil  a A R' ->
       ~ AtomSetImpl.In  F  (dom  S )  ->
-     Sig  (( F ~ Ax a A )++ S ) .
+      ( SubRole R' R )  ->
+     Sig  (( F ~ Ax a A R' )++ S ) .
 
 (* defns Jann *)
 Inductive AnnPropWff : context -> constraint -> Prop :=    (* defn AnnPropWff *)
- | An_Wff : forall (G:context) (a b A B:tm),
-     AnnTyping G a A ->
-     AnnTyping G b B ->
+ | An_Wff : forall (G:context) (a b A:tm) (R:role) (B:tm),
+     AnnTyping G a A R ->
+     AnnTyping G b B R ->
       (  (erase_tm  A )   =   (erase_tm  B )  )  ->
-     AnnPropWff G (Eq a b A)
-with AnnTyping : context -> tm -> tm -> Prop :=    (* defn AnnTyping *)
- | An_Star : forall (G:context),
+     AnnPropWff G (Eq a b A R)
+with AnnTyping : context -> tm -> tm -> role -> Prop :=    (* defn AnnTyping *)
+ | An_Star : forall (G:context) (R:role),
      AnnCtx G ->
-     AnnTyping G a_Star a_Star
- | An_Var : forall (G:context) (x:tmvar) (A:tm),
+     AnnTyping G a_Star a_Star R
+ | An_Var : forall (G:context) (x:tmvar) (A:tm) (R:role),
      AnnCtx G ->
-      binds  x  (Tm  A )  G  ->
-     AnnTyping G (a_Var_f x) A
- | An_Pi : forall (L:vars) (G:context) (rho:relflag) (A B:tm),
-      ( forall x , x \notin  L  -> AnnTyping  (( x ~ Tm  A ) ++  G )   ( open_tm_wrt_tm B (a_Var_f x) )  a_Star )  ->
-      ( AnnTyping G A a_Star )  ->
-     AnnTyping G (a_Pi rho A B) a_Star
- | An_Abs : forall (L:vars) (G:context) (rho:relflag) (A a B:tm),
-      ( AnnTyping G A a_Star )  ->
-      ( forall x , x \notin  L  -> AnnTyping  (( x ~ Tm  A ) ++  G )   ( open_tm_wrt_tm a (a_Var_f x) )   ( open_tm_wrt_tm B (a_Var_f x) )  )  ->
+      binds  x  (Tm  A R )  G  ->
+     AnnTyping G (a_Var_f x) A R
+ | An_Pi : forall (L:vars) (G:context) (rho:relflag) (A:tm) (R:role) (B:tm) (R':role),
+      ( forall x , x \notin  L  -> AnnTyping  (( x ~ Tm  A R ) ++  G )   ( open_tm_wrt_tm B (a_Var_f x) )  a_Star R' )  ->
+      ( AnnTyping G A a_Star R )  ->
+     AnnTyping G (a_Pi rho A R B) a_Star R'
+ | An_Abs : forall (L:vars) (G:context) (rho:relflag) (A:tm) (R:role) (a B:tm) (R':role),
+      ( AnnTyping G A a_Star R )  ->
+      ( forall x , x \notin  L  -> AnnTyping  (( x ~ Tm  A R ) ++  G )   ( open_tm_wrt_tm a (a_Var_f x) )   ( open_tm_wrt_tm B (a_Var_f x) )  R' )  ->
       ( forall x , x \notin  L  -> RhoCheck rho x  (erase_tm   ( open_tm_wrt_tm a (a_Var_f x) )  )  )  ->
-     AnnTyping G (a_Abs rho A a) (a_Pi rho A B)
- | An_App : forall (G:context) (b:tm) (rho:relflag) (a B A:tm),
-     AnnTyping G b (a_Pi rho A B) ->
-     AnnTyping G a A ->
-     AnnTyping G (a_App b rho a)  (open_tm_wrt_tm  B   a ) 
- | An_Conv : forall (G:context) (a:tm) (g:co) (B A:tm),
-     AnnTyping G a A ->
-     AnnDefEq G  (dom  G )  g A B ->
-     AnnTyping G B a_Star ->
-     AnnTyping G (a_Conv a g) B
- | An_CPi : forall (L:vars) (G:context) (phi:constraint) (B:tm),
+     SubRole R R' ->
+     AnnTyping G (a_Abs rho A R a)  ( (a_Pi rho A R B) )  R'
+ | An_App : forall (G:context) (b:tm) (rho:relflag) (a B:tm) (R':role) (A:tm) (R:role),
+     AnnTyping G b  ( (a_Pi rho A R B) )  R' ->
+     AnnTyping G a A R ->
+     AnnTyping G (a_App b rho a)  (  (open_tm_wrt_tm  B   a )  )  R'
+ | An_Conv : forall (G:context) (a:tm) (g:co) (B:tm) (R:role) (A:tm),
+     AnnTyping G a A R ->
+     AnnDefEq G  (dom  G )  g A B R ->
+     AnnTyping G B a_Star R ->
+     AnnTyping G (a_Conv a g) B R
+ | An_CPi : forall (L:vars) (G:context) (phi:constraint) (B:tm) (R:role),
       ( AnnPropWff G phi )  ->
-      ( forall c , c \notin  L  -> AnnTyping  (( c ~ Co  phi ) ++  G )   ( open_tm_wrt_co B (g_Var_f c) )  a_Star )  ->
-     AnnTyping G (a_CPi phi B) a_Star
- | An_CAbs : forall (L:vars) (G:context) (phi:constraint) (a B:tm),
+      ( forall c , c \notin  L  -> AnnTyping  (( c ~ Co  phi ) ++  G )   ( open_tm_wrt_co B (g_Var_f c) )  a_Star R )  ->
+     AnnTyping G (a_CPi phi B) a_Star R
+ | An_CAbs : forall (L:vars) (G:context) (phi:constraint) (a B:tm) (R:role),
       ( AnnPropWff G phi )  ->
-      ( forall c , c \notin  L  -> AnnTyping  (( c ~ Co  phi ) ++  G )   ( open_tm_wrt_co a (g_Var_f c) )   ( open_tm_wrt_co B (g_Var_f c) )  )  ->
-     AnnTyping G (a_CAbs phi a) (a_CPi phi B)
- | An_CApp : forall (G:context) (a1:tm) (g:co) (B a b A1:tm),
-     AnnTyping G a1 (a_CPi (Eq a b A1) B) ->
-     AnnDefEq G  (dom  G )  g a b ->
-     AnnTyping G (a_CApp a1 g)  (open_tm_wrt_co  B   g ) 
- | An_Fam : forall (G:context) (F:tyfam) (A a:tm),
+      ( forall c , c \notin  L  -> AnnTyping  (( c ~ Co  phi ) ++  G )   ( open_tm_wrt_co a (g_Var_f c) )   ( open_tm_wrt_co B (g_Var_f c) )  R )  ->
+     AnnTyping G (a_CAbs phi a)  ( (a_CPi phi B) )  R
+ | An_CApp : forall (G:context) (a1:tm) (g:co) (B:tm) (R':role) (a b A1:tm) (R:role),
+     AnnTyping G a1  ( (a_CPi (Eq a b A1 R) B) )  R' ->
+     AnnDefEq G  (dom  G )  g a b R ->
+     AnnTyping G (a_CApp a1 g)  (open_tm_wrt_co  B   g )  R'
+ | An_Fam : forall (G:context) (F:tyfam) (A:tm) (R:role) (a:tm),
      AnnCtx G ->
-      binds  F  (Ax  a A )   an_toplevel   ->
-      ( AnnTyping  nil  A a_Star )  ->
-     AnnTyping G (a_Fam F) A
+      binds  F  (Ax  a A R )   an_toplevel   ->
+      ( AnnTyping  nil  A a_Star R )  ->
+     AnnTyping G (a_Fam F) A R
 with AnnIso : context -> available_props -> co -> constraint -> constraint -> Prop :=    (* defn AnnIso *)
- | An_PropCong : forall (G:context) (D:available_props) (g1:co) (A:tm) (g2:co) (A1 B1 A2 B2:tm),
-     AnnDefEq G D g1 A1 A2 ->
-     AnnDefEq G D g2 B1 B2 ->
-     AnnPropWff G (Eq A1 B1 A) ->
-     AnnPropWff G (Eq A2 B2 A) ->
-     AnnIso G D  ( (g_EqCong g1 A g2) )   ( (Eq A1 B1 A) )   ( (Eq A2 B2 A) ) 
- | An_CPiFst : forall (G:context) (D:available_props) (g:co) (phi1 phi2:constraint) (A2 B2:tm),
-     AnnDefEq G D g (a_CPi phi1 A2) (a_CPi phi2 B2) ->
+ | An_PropCong : forall (G:context) (D:available_props) (g1:co) (A:tm) (R:role) (g2:co) (A1 B1 A2 B2:tm),
+     AnnDefEq G D g1 A1 A2 R ->
+     AnnDefEq G D g2 B1 B2 R ->
+     AnnPropWff G (Eq A1 B1 A R) ->
+     AnnPropWff G (Eq A2 B2 A R) ->
+     AnnIso G D  ( (g_EqCong g1 A R g2) )   ( (Eq A1 B1 A R) )   ( (Eq A2 B2 A R) ) 
+ | An_CPiFst : forall (G:context) (D:available_props) (g:co) (phi1 phi2:constraint) (A2 B2:tm) (R:role),
+     AnnDefEq G D g (a_CPi phi1 A2) (a_CPi phi2 B2) R ->
      AnnIso G D (g_CPiFst g) phi1 phi2
  | An_IsoSym : forall (G:context) (D:available_props) (g:co) (phi2 phi1:constraint),
      AnnIso G D g phi1 phi2 ->
      AnnIso G D (g_Sym g) phi2 phi1
- | An_IsoConv : forall (G:context) (D:available_props) (a1 a2 A a1' a2' B:tm) (g:co),
-     AnnDefEq G D g A B ->
-     AnnPropWff G (Eq a1 a2 A) ->
-     AnnPropWff G (Eq a1' a2' B) ->
+ | An_IsoConv : forall (G:context) (D:available_props) (a1 a2 A:tm) (R:role) (a1' a2' B:tm) (g:co),
+     AnnDefEq G D g A B R ->
+     AnnPropWff G (Eq a1 a2 A R) ->
+     AnnPropWff G (Eq a1' a2' B R) ->
       (  (erase_tm  a1 )   =   (erase_tm  a1' )  )  ->
       (  (erase_tm  a2 )   =   (erase_tm  a2' )  )  ->
-     AnnIso G D (g_IsoConv  ( (Eq a1 a2 A) )   ( (Eq a1' a2' B) )  g)  ( (Eq a1 a2 A) )   ( (Eq a1' a2' B) ) 
-with AnnDefEq : context -> available_props -> co -> tm -> tm -> Prop :=    (* defn AnnDefEq *)
- | An_Assn : forall (G:context) (D:available_props) (c:covar) (a b A:tm),
+     AnnIso G D (g_IsoConv  ( (Eq a1 a2 A R) )   ( (Eq a1' a2' B R) )  g)  ( (Eq a1 a2 A R) )   ( (Eq a1' a2' B R) ) 
+with AnnDefEq : context -> available_props -> co -> tm -> tm -> role -> Prop :=    (* defn AnnDefEq *)
+ | An_Assn : forall (G:context) (D:available_props) (c:covar) (a b:tm) (R:role) (A:tm),
      AnnCtx G ->
-      binds  c  (Co  (Eq a b A) )  G  ->
+      binds  c  (Co  (Eq a b A R) )  G  ->
       AtomSetImpl.In  c   D  ->
-     AnnDefEq G D (g_Var_f c) a b
- | An_Refl : forall (G:context) (D:available_props) (a A:tm),
-     AnnTyping G a A ->
-     AnnDefEq G D (g_Refl a) a a
- | An_EraseEq : forall (G:context) (D:available_props) (a b:tm) (g:co) (A B:tm),
-     AnnTyping G a A ->
-     AnnTyping G b B ->
+     AnnDefEq G D (g_Var_f c) a b R
+ | An_Refl : forall (G:context) (D:available_props) (a:tm) (R:role) (A:tm),
+     AnnTyping G a A R ->
+     AnnDefEq G D (g_Refl a) a a R
+ | An_EraseEq : forall (G:context) (D:available_props) (a b:tm) (g:co) (R:role) (A B:tm),
+     AnnTyping G a A R ->
+     AnnTyping G b B R ->
       (  (erase_tm  a )   =   (erase_tm  b )  )  ->
-     AnnDefEq G  (dom  G )  g A B ->
-     AnnDefEq G D (g_Refl2 a b g) a b
- | An_Sym : forall (G:context) (D:available_props) (g:co) (a b B A:tm) (g1:co),
-     AnnTyping G b B ->
-     AnnTyping G a A ->
-      ( AnnDefEq G  (dom  G )  g1 B A )  ->
-     AnnDefEq G D g b a ->
-     AnnDefEq G D (g_Sym g) a b
- | An_Trans : forall (G:context) (D:available_props) (g1 g2:co) (a b a1 A A1:tm) (g3:co),
-     AnnDefEq G D g1 a a1 ->
-     AnnDefEq G D g2 a1 b ->
-      ( AnnTyping G a A )  ->
-      ( AnnTyping G a1 A1 )  ->
-      ( AnnDefEq G  (dom  G )  g3 A A1 )  ->
-     AnnDefEq G D  ( (g_Trans g1 g2) )  a b
- | An_Beta : forall (G:context) (D:available_props) (a1 a2 B0 B1:tm),
-     AnnTyping G a1 B0 ->
-     AnnTyping G a2 B1 ->
+     AnnDefEq G  (dom  G )  g A B R ->
+     AnnDefEq G D (g_Refl2 a b g) a b R
+ | An_Sym : forall (G:context) (D:available_props) (g:co) (a b:tm) (R:role) (B A:tm) (g1:co),
+     AnnTyping G b B R ->
+     AnnTyping G a A R ->
+      ( AnnDefEq G  (dom  G )  g1 B A R )  ->
+     AnnDefEq G D g b a R ->
+     AnnDefEq G D (g_Sym g) a b R
+ | An_Trans : forall (G:context) (D:available_props) (g1 g2:co) (a b:tm) (R:role) (a1 A A1:tm) (g3:co),
+     AnnDefEq G D g1 a a1 R ->
+     AnnDefEq G D g2 a1 b R ->
+      ( AnnTyping G a A R )  ->
+      ( AnnTyping G a1 A1 R )  ->
+      ( AnnDefEq G  (dom  G )  g3 A A1 R )  ->
+     AnnDefEq G D  ( (g_Trans g1 g2) )  a b R
+ | An_Beta : forall (G:context) (D:available_props) (a1 a2:tm) (R:role) (B0 B1:tm),
+     AnnTyping G a1 B0 R ->
+     AnnTyping G a2 B1 R ->
       (  (erase_tm  B0 )   =   (erase_tm  B1 )  )  ->
      Beta  (erase_tm  a1 )   (erase_tm  a2 )  ->
-     AnnDefEq G D (g_Beta a1 a2) a1 a2
- | An_PiCong : forall (L:vars) (G:context) (D:available_props) (rho:relflag) (g1 g2:co) (A1 B1 A2 B3 B2:tm),
-     AnnDefEq G D g1 A1 A2 ->
-      ( forall x , x \notin  L  -> AnnDefEq  (( x ~ Tm  A1 ) ++  G )  D  ( open_co_wrt_tm g2 (a_Var_f x) )   ( open_tm_wrt_tm B1 (a_Var_f x) )    (open_tm_wrt_tm  B2   (a_Var_f x) )   )  ->
+     AnnDefEq G D (g_Beta a1 a2) a1 a2 R
+ | An_PiCong : forall (L:vars) (G:context) (D:available_props) (rho:relflag) (g1 g2:co) (A1:tm) (R:role) (B1 A2 B3 B2:tm),
+     AnnDefEq G D g1 A1 A2 R ->
+      ( forall x , x \notin  L  -> AnnDefEq  (( x ~ Tm  A1 R ) ++  G )  D  ( open_co_wrt_tm g2 (a_Var_f x) )   ( open_tm_wrt_tm B1 (a_Var_f x) )    (open_tm_wrt_tm  B2   (a_Var_f x) )   R )  ->
       ( forall x , x \notin  L  ->  (  ( open_tm_wrt_tm B3 (a_Var_f x) )   =   (open_tm_wrt_tm  B2   (a_Conv (a_Var_f x) (g_Sym g1)) )  )  )  ->
-     AnnTyping G (a_Pi rho A1 B1) a_Star ->
-     AnnTyping G (a_Pi rho A1 B2) a_Star ->
-     AnnTyping G (a_Pi rho A2 B3) a_Star ->
-     AnnDefEq G D (g_PiCong rho g1 g2)  ( (a_Pi rho A1 B1) )   ( (a_Pi rho A2 B3) ) 
- | An_AbsCong : forall (L:vars) (G:context) (D:available_props) (rho:relflag) (g1 g2:co) (A1 b1 A2 b3 b2 B:tm),
-     AnnDefEq G D g1 A1 A2 ->
-      ( forall x , x \notin  L  -> AnnDefEq  (( x ~ Tm  A1 ) ++  G )  D  ( open_co_wrt_tm g2 (a_Var_f x) )   ( open_tm_wrt_tm b1 (a_Var_f x) )    (open_tm_wrt_tm  b2   (a_Var_f x) )   )  ->
+     AnnTyping G (a_Pi rho A1 R B1) a_Star R ->
+     AnnTyping G (a_Pi rho A1 R B2) a_Star R ->
+     AnnTyping G (a_Pi rho A2 R B3) a_Star R ->
+     AnnDefEq G D (g_PiCong rho g1 g2)  ( (a_Pi rho A1 R B1) )   ( (a_Pi rho A2 R B3) )  R
+ | An_AbsCong : forall (L:vars) (G:context) (D:available_props) (rho:relflag) (g1 g2:co) (A1:tm) (R:role) (b1 A2 b3:tm) (R':role) (b2 B:tm),
+     AnnDefEq G D g1 A1 A2 R ->
+      ( forall x , x \notin  L  -> AnnDefEq  (( x ~ Tm  A1 R ) ++  G )  D  ( open_co_wrt_tm g2 (a_Var_f x) )   ( open_tm_wrt_tm b1 (a_Var_f x) )    (open_tm_wrt_tm  b2   (a_Var_f x) )   R' )  ->
       ( forall x , x \notin  L  ->  (  ( open_tm_wrt_tm b3 (a_Var_f x) )   =   (open_tm_wrt_tm  b2   (a_Conv (a_Var_f x) (g_Sym g1)) )  )  )  ->
-      ( AnnTyping G A1 a_Star )  ->
-     AnnTyping G A2 a_Star ->
+      ( AnnTyping G A1 a_Star R )  ->
+     AnnTyping G A2 a_Star R ->
       ( forall x , x \notin  L  -> RhoCheck rho x  (erase_tm   ( open_tm_wrt_tm b1 (a_Var_f x) )  )  )  ->
       ( forall x , x \notin  L  -> RhoCheck rho x  (erase_tm   ( open_tm_wrt_tm b3 (a_Var_f x) )  )  )  ->
-      ( AnnTyping G  ( (a_Abs rho A1 b2) )  B )  ->
-     AnnDefEq G D  ( (g_AbsCong rho g1 g2) )   ( (a_Abs rho A1 b1) )   ( (a_Abs rho A2 b3) ) 
- | An_AppCong : forall (G:context) (D:available_props) (g1:co) (rho:relflag) (g2:co) (a1 a2 b1 b2 A B:tm) (g3:co),
-     AnnDefEq G D g1 a1 b1 ->
-     AnnDefEq G D g2 a2 b2 ->
-     AnnTyping G (a_App a1 rho a2) A ->
-     AnnTyping G (a_App b1 rho b2) B ->
-      ( AnnDefEq G  (dom  G )  g3 A B )  ->
-     AnnDefEq G D (g_AppCong g1 rho g2) (a_App a1 rho a2) (a_App b1 rho b2)
- | An_PiFst : forall (G:context) (D:available_props) (g:co) (A1 A2:tm) (rho:relflag) (B1 B2:tm),
-     AnnDefEq G D g (a_Pi rho A1 B1) (a_Pi rho A2 B2) ->
-     AnnDefEq G D (g_PiFst g) A1 A2
- | An_PiSnd : forall (G:context) (D:available_props) (g1 g2:co) (B1 a1 B2 a2:tm) (rho:relflag) (A1 A2:tm),
-     AnnDefEq G D g1 (a_Pi rho A1 B1) (a_Pi rho A2 B2) ->
-     AnnDefEq G D g2 a1 a2 ->
-     AnnTyping G a1 A1 ->
-     AnnTyping G a2 A2 ->
-     AnnDefEq G D (g_PiSnd g1 g2)   (open_tm_wrt_tm  B1   a1 )     (open_tm_wrt_tm  B2   a2 )  
- | An_CPiCong : forall (L:vars) (G:context) (D:available_props) (g1 g3:co) (phi1:constraint) (B1:tm) (phi2:constraint) (B3 B2:tm),
+      ( AnnTyping G  ( (a_Abs rho A1 R b2) )  B R' )  ->
+      ( SubRole R R' )  ->
+     AnnDefEq G D  ( (g_AbsCong rho g1 g2) )   ( (a_Abs rho A1 R b1) )   ( (a_Abs rho A2 R b3) )  R'
+ | An_AppCong : forall (G:context) (D:available_props) (g1:co) (rho:relflag) (g2:co) (a1 a2 b1 b2:tm) (R' R:role) (A B:tm) (g3:co),
+     AnnDefEq G D g1 a1 b1 R' ->
+     AnnDefEq G D g2 a2 b2 R ->
+     AnnTyping G (a_App a1 rho a2) A R' ->
+     AnnTyping G (a_App b1 rho b2) B R' ->
+      ( AnnDefEq G  (dom  G )  g3 A B R' )  ->
+      ( SubRole R R' )  ->
+     AnnDefEq G D (g_AppCong g1 rho g2) (a_App a1 rho a2) (a_App b1 rho b2) R'
+ | An_PiFst : forall (G:context) (D:available_props) (g:co) (A1 A2:tm) (R3:role) (rho:relflag) (R1:role) (B1:tm) (R2:role) (B2:tm) (R:role),
+     AnnDefEq G D g (a_Pi rho A1 R1 B1) (a_Pi rho A2 R2 B2) R ->
+     SubRole R3 R1 ->
+     SubRole R3 R2 ->
+     AnnDefEq G D (g_PiFst g) A1 A2 R3
+ | An_PiSnd : forall (G:context) (D:available_props) (g1 g2:co) (B1 a1 B2 a2:tm) (R':role) (rho:relflag) (A1:tm) (R1:role) (A2:tm) (R2 R:role),
+     AnnDefEq G D g1 (a_Pi rho A1 R1 B1) (a_Pi rho A2 R2 B2) R' ->
+     AnnDefEq G D g2 a1 a2 R ->
+     AnnTyping G a1 A1 R ->
+     AnnTyping G a2 A2 R ->
+     SubRole R R1 ->
+     SubRole R R2 ->
+     AnnDefEq G D (g_PiSnd g1 g2)   (open_tm_wrt_tm  B1   a1 )     (open_tm_wrt_tm  B2   a2 )   R'
+ | An_CPiCong : forall (L:vars) (G:context) (D:available_props) (g1 g3:co) (phi1:constraint) (B1:tm) (phi2:constraint) (B3:tm) (R:role) (B2:tm),
      AnnIso G D g1 phi1 phi2 ->
-      ( forall c , c \notin  L  -> AnnDefEq  (( c ~ Co  phi1 ) ++  G )  D  ( open_co_wrt_co g3 (g_Var_f c) )   ( open_tm_wrt_co B1 (g_Var_f c) )    (open_tm_wrt_co  B2   (g_Var_f c) )   )  ->
+      ( forall c , c \notin  L  -> AnnDefEq  (( c ~ Co  phi1 ) ++  G )  D  ( open_co_wrt_co g3 (g_Var_f c) )   ( open_tm_wrt_co B1 (g_Var_f c) )    (open_tm_wrt_co  B2   (g_Var_f c) )   R )  ->
       ( forall c , c \notin  L  ->  (  ( open_tm_wrt_co B3 (g_Var_f c) )   =   (open_tm_wrt_co  B2   (g_Cast (g_Var_f c) (g_Sym g1)) )  )  )  ->
-     AnnTyping G (a_CPi phi1 B1) a_Star ->
-      ( AnnTyping G (a_CPi phi2 B3) a_Star )  ->
-     AnnTyping G (a_CPi phi1 B2) a_Star ->
-     AnnDefEq G D  ( (g_CPiCong g1 g3) )   ( (a_CPi phi1 B1) )   ( (a_CPi phi2 B3) ) 
- | An_CAbsCong : forall (L:vars) (G:context) (D:available_props) (g1 g3 g4:co) (phi1:constraint) (a1:tm) (phi2:constraint) (a3 a2 B1 B B2:tm),
+     AnnTyping G (a_CPi phi1 B1) a_Star R ->
+      ( AnnTyping G (a_CPi phi2 B3) a_Star R )  ->
+     AnnTyping G (a_CPi phi1 B2) a_Star R ->
+     AnnDefEq G D  ( (g_CPiCong g1 g3) )   ( (a_CPi phi1 B1) )   ( (a_CPi phi2 B3) )  R
+ | An_CAbsCong : forall (L:vars) (G:context) (D:available_props) (g1 g3 g4:co) (phi1:constraint) (a1:tm) (phi2:constraint) (a3:tm) (R:role) (a2 B1 B B2:tm),
      AnnIso G D g1 phi1 phi2 ->
-      ( forall c , c \notin  L  -> AnnDefEq  (( c ~ Co  phi1 ) ++  G )  D  ( open_co_wrt_co g3 (g_Var_f c) )   ( open_tm_wrt_co a1 (g_Var_f c) )    (open_tm_wrt_co  a2   (g_Var_f c) )   )  ->
+      ( forall c , c \notin  L  -> AnnDefEq  (( c ~ Co  phi1 ) ++  G )  D  ( open_co_wrt_co g3 (g_Var_f c) )   ( open_tm_wrt_co a1 (g_Var_f c) )    (open_tm_wrt_co  a2   (g_Var_f c) )   R )  ->
       ( forall c , c \notin  L  ->  (  ( open_tm_wrt_co a3 (g_Var_f c) )   =   (open_tm_wrt_co  a2   (g_Cast (g_Var_f c) (g_Sym g1)) )  )  )  ->
-     AnnTyping G  ( (a_CAbs phi1 a1) )  (a_CPi phi1 B1) ->
-     AnnTyping G  ( (a_CAbs phi1 a2) )  B ->
-     AnnTyping G  ( (a_CAbs phi2 a3) )  (a_CPi phi2 B2) ->
-     AnnDefEq G  (dom  G )  g4 (a_CPi phi1 B1) (a_CPi phi2 B2) ->
-     AnnDefEq G D  ( (g_CAbsCong g1 g3 g4) )   ( (a_CAbs phi1 a1) )   ( (a_CAbs phi2 a3) ) 
- | An_CAppCong : forall (G:context) (D:available_props) (g1 g2 g3:co) (a1 b1 a2 b2 a3 b3 A B:tm) (g4:co),
-     AnnDefEq G D g1 a1 b1 ->
-     AnnDefEq G  (dom  G )  g2 a2 b2 ->
-     AnnDefEq G  (dom  G )  g3 a3 b3 ->
-     AnnTyping G (a_CApp a1 g2) A ->
-     AnnTyping G (a_CApp b1 g3) B ->
-      ( AnnDefEq G  (dom  G )  g4 A B )  ->
-     AnnDefEq G D (g_CAppCong g1 g2 g3) (a_CApp a1 g2) (a_CApp b1 g3)
- | An_CPiSnd : forall (G:context) (D:available_props) (g1 g2 g3:co) (B1 B2 a a' A b b' B:tm),
-     AnnDefEq G D g1  ( (a_CPi (Eq a a' A) B1) )   ( (a_CPi (Eq b b' B) B2) )  ->
-     AnnDefEq G  (dom  G )  g2 a a' ->
-     AnnDefEq G  (dom  G )  g3 b b' ->
-     AnnDefEq G D (g_CPiSnd g1 g2 g3)  (open_tm_wrt_co  B1   g2 )   (open_tm_wrt_co  B2   g3 ) 
- | An_Cast : forall (G:context) (D:available_props) (g1 g2:co) (b b' a a' A B:tm),
-     AnnDefEq G D g1 a a' ->
-     AnnIso G D g2 (Eq a a' A) (Eq b b' B) ->
-     AnnDefEq G D (g_Cast g1 g2) b b'
- | An_IsoSnd : forall (G:context) (D:available_props) (g:co) (A B a a' b b':tm),
-     AnnIso G D g  ( (Eq a a' A) )   ( (Eq b b' B) )  ->
-     AnnDefEq G D (g_IsoSnd g) A B
+     AnnTyping G  ( (a_CAbs phi1 a1) )  (a_CPi phi1 B1) R ->
+     AnnTyping G  ( (a_CAbs phi1 a2) )  B R ->
+     AnnTyping G  ( (a_CAbs phi2 a3) )  (a_CPi phi2 B2) R ->
+     AnnDefEq G  (dom  G )  g4 (a_CPi phi1 B1) (a_CPi phi2 B2) R ->
+     AnnDefEq G D  ( (g_CAbsCong g1 g3 g4) )   ( (a_CAbs phi1 a1) )   ( (a_CAbs phi2 a3) )  R
+ | An_CAppCong : forall (G:context) (D:available_props) (g1 g2 g3:co) (a1 b1:tm) (R:role) (a2 b2:tm) (R':role) (a3 b3 A B:tm) (g4:co),
+     AnnDefEq G D g1 a1 b1 R ->
+     AnnDefEq G  (dom  G )  g2 a2 b2 R' ->
+     AnnDefEq G  (dom  G )  g3 a3 b3 R' ->
+     AnnTyping G (a_CApp a1 g2) A R ->
+     AnnTyping G (a_CApp b1 g3) B R ->
+      ( AnnDefEq G  (dom  G )  g4 A B R )  ->
+     AnnDefEq G D (g_CAppCong g1 g2 g3) (a_CApp a1 g2) (a_CApp b1 g3) R
+ | An_CPiSnd : forall (G:context) (D:available_props) (g1 g2 g3:co) (B1 B2:tm) (R0:role) (a a' A:tm) (R:role) (b b' B:tm) (R':role),
+     AnnDefEq G D g1  ( (a_CPi (Eq a a' A R) B1) )   ( (a_CPi (Eq b b' B R') B2) )  R0 ->
+     AnnDefEq G  (dom  G )  g2 a a' R ->
+     AnnDefEq G  (dom  G )  g3 b b' R' ->
+     AnnDefEq G D (g_CPiSnd g1 g2 g3)  (open_tm_wrt_co  B1   g2 )   (open_tm_wrt_co  B2   g3 )  R0
+ | An_Cast : forall (G:context) (D:available_props) (g1 g2:co) (b b':tm) (R2:role) (a a':tm) (R1:role) (A B:tm),
+     AnnDefEq G D g1 a a' R1 ->
+     AnnIso G D g2 (Eq a a' A R1) (Eq b b' B R2) ->
+     AnnDefEq G D (g_Cast g1 g2) b b' R2
+ | An_IsoSnd : forall (G:context) (D:available_props) (g:co) (A B:tm) (R0:role) (a a':tm) (R1:role) (b b':tm) (R2:role),
+     AnnIso G D g  ( (Eq a a' A R1) )   ( (Eq b b' B R2) )  ->
+     SubRole R1 R0 ->
+     SubRole R2 R0 ->
+     AnnDefEq G D (g_IsoSnd g) A B R0
 with AnnCtx : context -> Prop :=    (* defn AnnCtx *)
  | An_Empty : 
      AnnCtx  nil 
- | An_ConsTm : forall (G:context) (x:tmvar) (A:tm),
+ | An_ConsTm : forall (G:context) (x:tmvar) (A:tm) (R:role),
      AnnCtx G ->
-     AnnTyping G A a_Star ->
+     AnnTyping G A a_Star R ->
       ~ AtomSetImpl.In  x  (dom  G )  ->
-     AnnCtx  (( x ~ Tm  A ) ++  G ) 
+     AnnCtx  (( x ~ Tm  A R ) ++  G ) 
  | An_ConsCo : forall (G:context) (c:covar) (phi:constraint),
      AnnCtx G ->
      AnnPropWff G phi ->
@@ -1370,12 +1412,12 @@ with AnnCtx : context -> Prop :=    (* defn AnnCtx *)
 with AnnSig : sig -> Prop :=    (* defn AnnSig *)
  | An_Sig_Empty : 
      AnnSig  nil 
- | An_Sig_ConsAx : forall (S:sig) (F:tyfam) (a A:tm),
+ | An_Sig_ConsAx : forall (S:sig) (F:tyfam) (a A:tm) (R:role),
      AnnSig S ->
-     AnnTyping  nil  A a_Star ->
-     AnnTyping  nil  a A ->
+     AnnTyping  nil  A a_Star R ->
+     AnnTyping  nil  a A R ->
       ~ AtomSetImpl.In  F  (dom  S )  ->
-     AnnSig  (( F ~ Ax a A )++ S ) .
+     AnnSig  (( F ~ Ax a A R )++ S ) .
 
 (* defns Jred *)
 Inductive head_reduction : context -> tm -> tm -> Prop :=    (* defn head_reduction *)
@@ -1383,10 +1425,10 @@ Inductive head_reduction : context -> tm -> tm -> Prop :=    (* defn head_reduct
      lc_tm b ->
      head_reduction G a a' ->
      head_reduction G (a_App a rho b) (a_App a' rho b)
- | An_AppAbs : forall (G:context) (rho:relflag) (A w a:tm),
+ | An_AppAbs : forall (G:context) (rho:relflag) (A:tm) (R:role) (w a:tm),
      lc_tm a ->
-     Value  ( (a_Abs rho A w) )  ->
-     head_reduction G (a_App  ( (a_Abs rho A w) )  rho a)  (open_tm_wrt_tm  w   a ) 
+     Value  ( (a_Abs rho A R w) )  ->
+     head_reduction G (a_App  ( (a_Abs rho A R w) )  rho a)  (open_tm_wrt_tm  w   a ) 
  | An_CAppLeft : forall (G:context) (a:tm) (g:co) (a':tm),
      lc_co g ->
      head_reduction G a a' ->
@@ -1396,12 +1438,12 @@ Inductive head_reduction : context -> tm -> tm -> Prop :=    (* defn head_reduct
      lc_tm (a_CAbs phi b) ->
      lc_co g ->
      head_reduction G (a_CApp  ( (a_CAbs phi b) )  g)  (open_tm_wrt_co  b   g ) 
- | An_AbsTerm : forall (L:vars) (G:context) (A b b':tm),
-     AnnTyping G A a_Star ->
-      ( forall x , x \notin  L  -> head_reduction  (( x ~ Tm  A ) ++  G )   ( open_tm_wrt_tm b (a_Var_f x) )   ( open_tm_wrt_tm b' (a_Var_f x) )  )  ->
-     head_reduction G  ( (a_Abs Irrel A b) )   ( (a_Abs Irrel A b') ) 
- | An_Axiom : forall (G:context) (F:tyfam) (a A:tm),
-      binds  F  (Ax  a A )   an_toplevel   ->
+ | An_AbsTerm : forall (L:vars) (G:context) (A:tm) (R:role) (b b':tm),
+     AnnTyping G A a_Star R ->
+      ( forall x , x \notin  L  -> head_reduction  (( x ~ Tm  A R ) ++  G )   ( open_tm_wrt_tm b (a_Var_f x) )   ( open_tm_wrt_tm b' (a_Var_f x) )  )  ->
+     head_reduction G  ( (a_Abs Irrel A R b) )   ( (a_Abs Irrel A R b') ) 
+ | An_Axiom : forall (G:context) (F:tyfam) (a A:tm) (R:role),
+      binds  F  (Ax  a A R )   an_toplevel   ->
      head_reduction G (a_Fam F) a
  | An_ConvTerm : forall (G:context) (a:tm) (g:co) (a':tm),
      lc_co g ->
@@ -1412,21 +1454,21 @@ Inductive head_reduction : context -> tm -> tm -> Prop :=    (* defn head_reduct
      lc_co g2 ->
      Value v ->
      head_reduction G (a_Conv  ( (a_Conv v g1) )  g2) (a_Conv v  ( (g_Trans g1 g2) ) )
- | An_Push : forall (G:context) (v:tm) (g:co) (rho:relflag) (b b':tm) (g':co) (A1 B1 A2 B2:tm),
+ | An_Push : forall (G:context) (v:tm) (g:co) (rho:relflag) (b b':tm) (g':co) (A1:tm) (R1:role) (B1 A2:tm) (R2:role) (B2:tm) (R:role),
      Value v ->
-     AnnDefEq G  (dom  G )  g (a_Pi rho A1 B1) (a_Pi rho A2 B2) ->
+     AnnDefEq G  (dom  G )  g (a_Pi rho A1 R1 B1) (a_Pi rho A2 R2 B2) R ->
       ( b'  =  (a_Conv b (g_Sym  ( (g_PiFst g) ) )) )  ->
       ( g'  =  (g_PiSnd g (g_Refl2 b' b  ( (g_PiFst g) ) )) )  ->
      head_reduction G (a_App  ( (a_Conv v g) )  rho b) (a_Conv  ( (a_App v rho b') )  g')
- | An_CPush : forall (G:context) (v:tm) (g g1 g1' g':co) (phi1:constraint) (A1:tm) (phi2:constraint) (A2:tm),
+ | An_CPush : forall (G:context) (v:tm) (g g1 g1' g':co) (phi1:constraint) (A1:tm) (phi2:constraint) (A2:tm) (R:role),
      Value v ->
-     AnnDefEq G  (dom  G )  g (a_CPi phi1 A1) (a_CPi phi2 A2) ->
+     AnnDefEq G  (dom  G )  g (a_CPi phi1 A1) (a_CPi phi2 A2) R ->
       ( g1'  =  (g_Cast g1 (g_Sym  ( (g_CPiFst g) ) )) )  ->
       ( g'  =  (g_CPiSnd g g1' g1) )  ->
      head_reduction G (a_CApp  ( (a_Conv v g) )  g1) (a_Conv  ( (a_CApp v g1') )  g').
 
 
 (** infrastructure *)
-Hint Constructors CoercedValue Value value_type consistent erased_tm RhoCheck Par MultiPar joins Beta reduction_in_one reduction PropWff Typing Iso DefEq Ctx Sig AnnPropWff AnnTyping AnnIso AnnDefEq AnnCtx AnnSig head_reduction lc_constraint lc_co lc_brs lc_tm lc_sort lc_sig_sort.
+Hint Constructors SubRole CoercedValue Value value_type consistent erased_tm RhoCheck Par MultiPar joins Beta reduction_in_one reduction PropWff Typing Iso DefEq Ctx Sig AnnPropWff AnnTyping AnnIso AnnDefEq AnnCtx AnnSig head_reduction lc_co lc_brs lc_tm lc_constraint lc_sort lc_sig_sort.
 
 
